examples/dynamic_isolation/Proof.v
@@ -60,6 +60,24 @@ Ltac destruct_one_var_with t :=
 Ltac destruct_vars_with t :=
   repeat (destruct_one_var_with t).
 
+Ltac solve' :=
+  match goal with
+  | |- ?x = (fst ?x, snd ?x) =>
+    destruct x; reflexivity
+  | [ H: False |- _ ] => solve [ destruct H ]
+  | [ H: ?P |- ?P ] => exact H
+  end.
+
+Ltac rewrite_in_goal :=
+  repeat lazymatch goal with
+  | H: ?x = ?x |- _ =>  fail 1
+  | H: ?x = _ |- context[?x] =>
+      rewrite H
+  end.
+
+Ltac simplify_tupless := simplify_tuples; subst.
+
+
 Tactic Notation "destruct_one_var" := destruct_one_var_with auto.
 Tactic Notation "destruct_vars_with" tactic(t) := repeat (destruct_one_var_with t).
 Tactic Notation "destruct_vars" := destruct_vars_with auto.
@@ -237,81 +255,6 @@ Tactic Notation "destruct_vars" := destruct_vars_with auto.
   Definition spec1_log_t : Type := Spec.Machine1.log_t.
 
   (* ================= END_TMP ====================== *)
-
-  (* Section GhostState. *)
-
-  (*   (* Experimenting with input/output state representation *) *)
-  (*   Inductive modules := *)
-  (*   | Module_Core0 *)
-  (*   | Module_Core1 *)
-  (*   | Module_SM *)
-  (*   | Module_Memory *)
-  (*   . *)
-
-  (*   Record ghost_state : Type. (* TODO *) *)
-
-  (*   Definition impl_ghost_state : Type. Admitted. *)
-  (*   Definition spec_ghost_state : Type. Admitted. *)
-
-  (*   Definition initial_impl_ghost : impl_ghost_state. Admitted. *)
-  (*   Definition initial_spec_ghost : spec_ghost_state. Admitted. *)
-
-  (*   Definition impl_step_with_ghost (st: Impl.state * impl_ghost_state) *)
-  (*                                   : (Impl.state * impl_ghost_state) * tau := *)
-  (*     let (impl_st, ghost_st) := st in *)
-  (*     ((fst (Impl.step impl_st), ghost_st (* TODO *)), (snd (Impl.step impl_st))). *)
-
-  (*   Definition spec_step_with_ghost (st: Spec.state * spec_ghost_state) *)
-  (*                                   : (Spec.state * spec_ghost_state) * tau := *)
-  (*     let (spec_st, ghost_st) := st in *)
-  (*     ((fst (Spec.step spec_st), ghost_st (* TODO *)), (snd (Spec.step spec_st))). *)
-
-  (*   Section Initialised. *)
-  (*     Context (initial_dram : dram_t). *)
-
-  (*     Definition impl_step_n_with_ghost (n: nat) : (Impl.state * impl_ghost_state) * trace := *)
-  (*       step_n (Impl.initial_state initial_dram, initial_impl_ghost) *)
-  (*              impl_step_with_ghost *)
-  (*              n. *)
-
-  (*     Definition spec_step_n_with_ghost (n: nat) : (Spec.state * spec_ghost_state) * trace := *)
-  (*       step_n (Spec.initial_state initial_dram, initial_spec_ghost) *)
-  (*              spec_step_with_ghost *)
-  (*              n. *)
-
-  (*   End Initialised. *)
-
-  (*   Section Lemmas. *)
-
-  (*     Lemma impl_drop_ghost : *)
-  (*       forall (initial_dram: dram_t) *)
-  (*         n st st' evs evs', *)
-  (*         impl_step_n_with_ghost initial_dram n = (st, evs) -> *)
-  (*         Impl.step_n initial_dram n = (st', evs') -> *)
-  (*         st' = fst st /\ evs = evs'. *)
-  (*     Proof. *)
-  (*       intro. eapply proj_step_fn_eq. *)
-  (*       - unfold is_proj; auto. *)
-  (*       - unfold natural_step_fn. unfold impl_step_with_ghost, is_proj. *)
-  (*         intros; destruct_all_matches. *)
-  (*     Qed. *)
-
-  (*     Lemma spec_drop_ghost : *)
-  (*       forall (initial_dram: dram_t) *)
-  (*         n st st' evs evs', *)
-  (*         spec_step_n_with_ghost initial_dram n = (st, evs) -> *)
-  (*         Spec.step_n initial_dram n = (st', evs') -> *)
-  (*         st' = fst st /\ evs = evs'. *)
-  (*     Proof. *)
-  (*       intro. eapply proj_step_fn_eq. *)
-  (*       - unfold is_proj; auto. *)
-  (*       - unfold natural_step_fn. unfold spec_step_with_ghost, is_proj. *)
-  (*         intros; destruct_all_matches. *)
-  (*     Qed. *)
-
-  (*   End Lemmas. *)
-
-  (* End GhostState. *)
 
   Section ImplRegisterMap.
     Definition impl_sm_clk : Impl.System.reg_t := Impl.System.SM_private (SM_Common.clk).
@@ -520,6 +463,35 @@ Tactic Notation "destruct_vars" := destruct_vars_with auto.
 
   End Derived_Mem.
 
+  Ltac unfold_core0_steps :=
+    consider core0_do_steps__koika;
+    consider core0_do_step_input__koika;
+    consider core0_do_steps__spec;
+    consider core0_do_step_trans_input__spec.
+
+  Ltac unfold_core1_steps :=
+    consider core1_do_steps__koika;
+    consider core1_do_step_input__koika;
+    consider core1_do_steps__spec;
+    consider core1_do_step_trans_input__spec.
+
+  Ltac unfold_sm_steps :=
+    consider Impl.System.SM.do_steps__impl;
+    consider Impl.System.SM.do_step_input__impl;
+    consider Impl.System.SM.do_steps__spec.
+
+  Ltac unfold_mem_steps :=
+    consider mem_do_steps__impl;
+    consider mem_do_step_input__impl;
+    consider mem_do_steps__spec.
+
+  Ltac unfold_all_steps :=
+    unfold_core0_steps;
+    unfold_core1_steps;
+    unfold_sm_steps;
+    unfold_mem_steps.
+
+
   Section ImplProjs.
     Definition get_impl_core0 : Impl.koika_state_t -> core0_state_t :=
       fun impl_st => proj_env Impl.System.Lift_core0 impl_st.
@@ -584,7 +556,7 @@ Tactic Notation "destruct_vars" := destruct_vars_with auto.
       { output_core0 : Log Core0.R ContextEnv
       ; output_core1 : Log Core1.R ContextEnv
       ; output_sm : Log SM_Common.R ContextEnv
-      ; output_mem : Log Memory.R ContextEnv * Memory.external_state_t
+      ; output_mem : Log Memory.R ContextEnv (* * Memory.external_state_t *)
       }.
 
     Definition trace := list tau.
@@ -690,7 +662,7 @@ Tactic Notation "destruct_vars" := destruct_vars_with auto.
         {| output_core0 := core0_output__local;
            output_core1 := core1_output__local;
            output_sm := sm_output__local ;
-           output_mem := (mem_output__local, ext_st)
+           output_mem := (mem_output__local) (*, ext_st) *)
         |} in
       (* Do feedback: reverse *)
       let mem_feedback__global := log_empty in
@@ -742,7 +714,7 @@ Tactic Notation "destruct_vars" := destruct_vars_with auto.
         let core0_log := lift_log Impl.System.Lift_core0 ev.(output_core0) in
         let core1_log := lift_log Impl.System.Lift_core1 ev.(output_core1) in
         let sm_log := lift_log Impl.System.Lift_sm ev.(output_sm) in
-        let mem_log := lift_log Impl.System.Lift_mem (fst ev.(output_mem)) in
+        let mem_log := lift_log Impl.System.Lift_mem ev.(output_mem) in
         (mem_log ++ sm_log ++ core1_log ++ core0_log)%log.
 
       Definition core0_function_of_decoupled_io__state (st: core0_state_t) (ios: list Core_Common.step_io) : Prop :=
@@ -770,18 +742,6 @@ Tactic Notation "destruct_vars" := destruct_vars_with auto.
         consider @sm_function_of_decoupled_io__state;
         consider @mem_function_of_decoupled_io__state.
 
-      Ltac unfold_core0_steps :=
-        consider core0_do_steps__koika;
-        consider core0_do_step_input__koika.
-      Ltac unfold_core1_steps :=
-        consider core1_do_steps__koika;
-        consider core1_do_step_input__koika.
-      Ltac unfold_sm_steps :=
-        consider Impl.System.SM.do_steps__impl;
-        consider Impl.System.SM.do_step_input__impl.
-      Ltac unfold_mem_steps :=
-        consider mem_do_steps__impl;
-        consider mem_do_step_input__impl.
 
       Lemma step_state_function_of_decoupled_ios :
         forall initial_dram st ios st' t io,
@@ -846,7 +806,7 @@ Tactic Notation "destruct_vars" := destruct_vars_with auto.
         core0_function_of_decoupled_io__trace (map output_core0 tr) (map step_io_core0 step_ios) /\
         core1_function_of_decoupled_io__trace (map output_core1 tr) (map step_io_core1 step_ios) /\
         sm_function_of_decoupled_io__trace (map output_sm tr) (map step_io_sm step_ios) /\
-        mem_function_of_decoupled_io__trace initial_dram (map fst (map output_mem tr)) (map step_io_mem step_ios).
+        mem_function_of_decoupled_io__trace initial_dram (map output_mem tr) (map step_io_mem step_ios).
 
       Ltac unfold_decoupled_ios__trace :=
         consider @core0_function_of_decoupled_io__trace;
@@ -921,6 +881,68 @@ Tactic Notation "destruct_vars" := destruct_vars_with auto.
           specialize IHn with (1 := eq_refl); propositional.
           eapply step_trace_function_of_decoupled_ios; eauto.
           eapply step_rel_decoupled_step__state; eauto.
+      Qed.
+
+      Theorem step_n_extract_ios :
+        forall (initial_dram: dram_t) (n: nat)
+          (st: state) (tr: trace),
+          step_n initial_dram n = (st, tr) ->
+          exists step_ios, step_n_with_metadata initial_dram n = (st, tr, step_ios).
+      Proof.
+        induction n.
+        - simpl; intros; simplify_tuples; subst.
+          exists []; auto.
+        - simpl; intros; destruct_all_matches; simplify_tuples; subst.
+          exists (l ++ [m]).
+          specialize IHn with (1 := eq_refl); propositional; simplify_tuples; subst.
+          consider do_step.
+          rewrite Heqp1 in *. simpl in *. simplify_tuples; subst.
+          auto.
+      Qed.
+
+      Ltac solve_extract_steps_from_metadata :=
+        let HStep := fresh in
+        intros *; intro HStep; unfold_all_steps;
+          specialize step_rel_decoupled_step__state with (1 := HStep); intro Hstate;
+          specialize step_rel_decoupled_step__trace with (1 := HStep); intro Htrace;
+          consider state_function_of_decoupled_ios;
+          consider trace_function_of_decoupled_ios;
+          propositional;
+          unfold_decoupled_ios__state;
+          unfold_decoupled_ios__trace;
+          unfold_all_steps;
+          rewrite_in_goal; solve'.
+
+      Corollary extract_core0_steps_from_metadata :
+        forall initial_dram n st tr io,
+        step_n_with_metadata initial_dram n = (st, tr, io) ->
+        core0_do_steps__koika (map step_io_core0 io) = (state_core0 st, map output_core0 tr).
+      Proof.
+        solve_extract_steps_from_metadata.
+      Qed.
+
+      Corollary extract_core1_steps_from_metadata :
+        forall initial_dram n st tr io,
+        step_n_with_metadata initial_dram n = (st, tr, io) ->
+        core1_do_steps__koika (map step_io_core1 io) = (state_core1 st, map output_core1 tr).
+      Proof.
+        solve_extract_steps_from_metadata.
+      Qed.
+
+      Corollary extract_sm_steps_from_metadata :
+        forall initial_dram n st tr io,
+        step_n_with_metadata initial_dram n = (st, tr, io) ->
+        Impl.System.SM.do_steps__impl (map step_io_sm io) = (state_sm st, map output_sm tr).
+      Proof.
+        solve_extract_steps_from_metadata.
+      Qed.
+
+      Corollary extract_mem_steps_from_metadata :
+        forall initial_dram n st tr io,
+        step_n_with_metadata initial_dram n = (st, tr, io) ->
+        mem_do_steps__impl initial_dram (map step_io_mem io) = (state_mem st, map output_mem tr).
+      Proof.
+        solve_extract_steps_from_metadata.
       Qed.
 
     End HelperLemmas.
@@ -1049,14 +1071,16 @@ Tactic Notation "destruct_vars" := destruct_vars_with auto.
             |} in
         (sm_input, sm_output__raw, sm_output__global, acc, mk_sm_step_io, sm_ghost).
 
-      Definition do_mem (st: mem_spec_state_t) (input_log: Log Impl.System.R ContextEnv)
+      Definition do_mem (st: mem_spec_state_t)
+                        (input_log: Log Impl.System.R ContextEnv)
                         (ghost: sm_ghost_output_t)
                         : Log Mem_Common.R_public ContextEnv *
                           (Log Mem_Common.R ContextEnv * Log Mem_Common.R ContextEnv) *
                           Log Impl.System.R ContextEnv * Log Impl.System.R ContextEnv *
                           (Log Mem_Common.R_public ContextEnv -> Mem_Common.ghost_io) :=
         let mem_input := Mem_Common.proj_log__pub (proj_log (REnv := ContextEnv) Impl.System.Lift_mem input_log) in
-        let mem_output__raw := mem_do_step_trans_input__spec st mem_input in
+        let mem_output__raw := mem_do_step_trans_input__spec
+                               st (mem_input, (ghost_output_config0 ghost, ghost_output_config1 ghost)) in
         let mem_output__local := combine_mem_public_output mem_output__raw in
         let mem_output__global := lift_log (REnv := ContextEnv) Impl.System.Lift_mem mem_output__local in
         let acc_mem := log_app mem_output__global input_log in
@@ -1176,17 +1200,6 @@ Tactic Notation "destruct_vars" := destruct_vars_with auto.
         consider @core1_function_of_decoupled_io__state;
         consider @sm_function_of_decoupled_io__state;
         consider @mem_function_of_decoupled_io__state.
-
-      Ltac unfold_core0_steps :=
-        consider core0_do_steps__spec;
-        consider core0_do_step_trans_input__spec.
-      Ltac unfold_core1_steps :=
-        consider core1_do_steps__spec;
-        consider core1_do_step_trans_input__spec.
-      Ltac unfold_sm_steps :=
-        consider Impl.System.SM.do_steps__spec.
-      Ltac unfold_mem_steps :=
-        consider mem_do_steps__spec.
 
       Lemma step_state_function_of_decoupled_ios :
         forall initial_dram st ios st' t io,
@@ -1328,106 +1341,117 @@ Tactic Notation "destruct_vars" := destruct_vars_with auto.
           eapply step_rel_decoupled_step__state; eauto.
       Qed.
 
+      Theorem step_n_extract_ios :
+        forall (initial_dram: dram_t) (n: nat)
+          (st: state) (tr: trace),
+          step_n initial_dram n = (st, tr) ->
+          exists step_ios, step_n_with_metadata initial_dram n = (st, tr, step_ios).
+      Proof.
+        induction n.
+        - simpl; intros; simplify_tuples; subst.
+          exists []; auto.
+        - simpl; intros; destruct_all_matches; simplify_tuples; subst.
+          exists (l ++ [m]).
+          specialize IHn with (1 := eq_refl); propositional; simplify_tuples; subst.
+          consider do_step.
+          rewrite Heqp1 in *. simpl in *. simplify_tuples; subst.
+          auto.
+      Qed.
+
+      Ltac solve_extract_steps_from_metadata :=
+        let Hmeta := fresh in
+        let Hsteps := fresh in
+        intros *; intro Hmeta;
+        specialize step_rel_decoupled_step__state with (1 := Hmeta); intro Hstate;
+        specialize step_rel_decoupled_step__trace with (1 := Hmeta); intro Htrace;
+        match goal with
+        | |- exists _, ?x = _ =>
+            let props := fresh in
+            destruct x as [[? ?] props] eqn:Hsteps; exists props
+        end;
+        consider state_function_of_decoupled_ios;
+        consider trace_function_of_decoupled_ios;
+        propositional;
+        unfold_decoupled_ios__state;
+        unfold_decoupled_ios__trace;
+        rewrite Hsteps in *; simpl in *;
+        subst; auto.
+
+      Corollary extract_core0_steps_from_metadata :
+        forall initial_dram n st tr io,
+        step_n_with_metadata initial_dram n = (st, tr, io) ->
+        exists props, core0_do_steps__spec (map step_io_core0 io) = (state_core0 st, map output_core0 tr, props).
+      Proof.
+        solve_extract_steps_from_metadata.
+      Qed.
+
+      Corollary extract_core1_steps_from_metadata :
+        forall initial_dram n st tr io,
+        step_n_with_metadata initial_dram n = (st, tr, io) ->
+        exists props, core1_do_steps__spec (map step_io_core1 io) = (state_core1 st, map output_core1 tr, props).
+      Proof.
+        solve_extract_steps_from_metadata.
+      Qed.
+
+      Corollary extract_sm_steps_from_metadata :
+        forall initial_dram n st tr io,
+        step_n_with_metadata initial_dram n = (st, tr, io) ->
+        exists props, Impl.System.SM.do_steps__spec (map fst (map step_io_sm io)) = (state_sm st, map output_sm tr, props).
+      Proof.
+        solve_extract_steps_from_metadata.
+      Qed.
+
+      Corollary extract_mem_steps_from_metadata :
+        forall initial_dram n st tr io,
+        step_n_with_metadata initial_dram n = (st, tr, io) ->
+        exists props, mem_do_steps__spec initial_dram (map step_io_mem io) = (state_mem st, map output_mem tr, props).
+      Proof.
+        solve_extract_steps_from_metadata.
+      Qed.
+
     End HelperLemmas.
+
+    Section Invariant.
+      Definition InvariantState (st: state) : Prop. Admitted.
+
+      Lemma initial_invariant : forall dram, InvariantState (initial_state dram).
+      Admitted.
+
+      Definition core0_P_prop (P_prop: list props_t -> Prop) io :=
+        P_prop (snd (core0_do_steps__spec io)).
+      Definition core1_P_prop (P_prop: list props_t -> Prop) io :=
+        P_prop (snd (core1_do_steps__spec io)).
+      Definition sm_P_prop (P_prop: list props_t -> Prop) io :=
+        P_prop (snd (Impl.System.SM.do_steps__spec io)).
+      Definition mem_P_prop (P_prop: list props_t -> Prop) dram io :=
+        P_prop (snd (mem_do_steps__spec dram io)).
+
+      Definition valid_P_prop (P_prop: list props_t -> Prop) (initial_dram: dram_t) spec_io :=
+        core0_P_prop P_prop (map step_io_core0 spec_io) /\
+        core1_P_prop P_prop (map step_io_core1 spec_io) /\
+        sm_P_prop P_prop (map fst (map step_io_sm spec_io)) /\
+        mem_P_prop P_prop initial_dram (map step_io_mem spec_io).
+
+      Definition valid_props initial_dram spec_io :=
+        valid_P_prop valid_inputs initial_dram spec_io /\
+        valid_P_prop valid_outputs initial_dram spec_io /\
+        valid_P_prop valid_feedbacks initial_dram spec_io.
+
+      Theorem step_n_invariant :
+        forall initial_dram n spec_st spec_tr spec_io,
+        ModSpec.step_n_with_metadata initial_dram n = (spec_st, spec_tr, spec_io) ->
+        InvariantState spec_st /\ valid_props initial_dram spec_io.
+      Admitted.
+
+    End Invariant.
 
   End ModSpec.
 
   Module Observations.
     Import Interfaces.Common.
     (* TODO: write this in a nicer way *)
-    (*
-    Definition observe_imem_req0 (log: Log Core0.R ContextEnv) : option (struct_t mem_req) :=
-      observe_enq0 (Core0.public (Core0.toIMem MemReq.valid0)) eq_refl
-                   (Core0.public (Core0.toIMem MemReq.data0)) eq_refl log.
-    Definition observe_dmem_req0 (log: Log Core0.R ContextEnv) : option (struct_t mem_req) :=
-      observe_enq0 (Core0.public (Core0.toDMem MemReq.valid0)) eq_refl
-                   (Core0.public (Core0.toDMem MemReq.data0)) eq_refl log.
-    Definition observe_imem_req1 (log: Log Core1.R ContextEnv) : option (struct_t mem_req) :=
-      observe_enq0 (Core1.public (Core1.toIMem MemReq.valid0)) eq_refl
-                   (Core1.public (Core1.toIMem MemReq.data0)) eq_refl log.
-    Definition observe_dmem_req1 (log: Log Core1.R ContextEnv) : option (struct_t mem_req) :=
-      observe_enq0 (Core1.public (Core1.toDMem MemReq.valid0)) eq_refl
-                   (Core1.public (Core1.toDMem MemReq.data0)) eq_refl log.
-    Definition observe_imem_resp0 (log: Log SM_Common.R ContextEnv) : option (struct_t mem_resp) :=
-      observe_enq1 (SM_Common.public (SM_Common.toCore0_IMem MemResp.valid0)) eq_refl
-                   (SM_Common.public (SM_Common.toCore0_IMem MemResp.data0)) eq_refl log.
-    Definition observe_dmem_resp0 (log: Log SM_Common.R ContextEnv) : option (struct_t mem_resp) :=
-      observe_enq1 (SM_Common.public (SM_Common.toCore0_DMem MemResp.valid0)) eq_refl
-                   (SM_Common.public (SM_Common.toCore0_DMem MemResp.data0)) eq_refl log.
-    Definition observe_imem_resp1 (log: Log SM_Common.R ContextEnv) : option (struct_t mem_resp) :=
-      observe_enq1 (SM_Common.public (SM_Common.toCore1_IMem MemResp.valid0)) eq_refl
-                   (SM_Common.public (SM_Common.toCore1_IMem MemResp.data0)) eq_refl log.
-    Definition observe_dmem_resp1 (log: Log SM_Common.R ContextEnv) : option (struct_t mem_resp) :=
-      observe_enq1 (SM_Common.public (SM_Common.toCore1_DMem MemResp.valid0)) eq_refl
-                   (SM_Common.public (SM_Common.toCore1_DMem MemResp.data0)) eq_refl log.
-    Definition observe_enclave_req0 (log: Log Core0.R ContextEnv) : option (struct_t enclave_req) :=
-      observe_enq0 (Core0.public (Core0.toSMEnc EnclaveReq.valid0)) eq_refl
-                   (Core0.public (Core0.toSMEnc EnclaveReq.data0)) eq_refl
-                   log.
-    Definition observe_enclave_req1 (log: Log Core1.R ContextEnv) : option (struct_t enclave_req) :=
-      observe_enq0 (Core1.public (Core1.toSMEnc EnclaveReq.valid0)) eq_refl
-                   (Core1.public (Core1.toSMEnc EnclaveReq.data0)) eq_refl
-                   log.
-    Definition observe_enclave_enter0 (log: Log SM_Common.R ContextEnv) : bool :=
-      match latest_write log (SM_Common.public SM_Common.purge_core0) with
-      | Some v => bits_eqb v ENUM_purge_restart
-      | None => false
-      end.
-    Definition observe_enclave_enter1 (log: Log SM_Common.R ContextEnv) : bool :=
-      match latest_write log (SM_Common.public SM_Common.purge_core1) with
-      | Some v => bits_eqb v ENUM_purge_restart
-      | None => false
-      end.
-    Definition observe_enclave_exit0 (log: Log SM_Common.R ContextEnv) : bool :=
-      match latest_write log (SM_Common.private SM_Common.enc_data0) with
-      | Some v =>
-          let data := EnclaveInterface.extract_enclave_data v in
-          bits_eqb (EnclaveInterface.enclave_data_valid data) Ob~0
-      | None => false
-      end.
-    Definition observe_enclave_exit1 (log: Log SM_Common.R ContextEnv) : bool :=
-      match latest_write log (SM_Common.private SM_Common.enc_data1) with
-      | Some v =>
-          let data := EnclaveInterface.extract_enclave_data v in
-          bits_eqb (EnclaveInterface.enclave_data_valid data) Ob~0
-      | None => false
-      end.
-      *)
-
     Definition generate_observations__modImpl (ev: ModImpl.tau) : tau :=
       fun core_id => Impl.do_observations (ModImpl.outputs_to_impl_log ev) core_id.
-
-        (*
-        let sm_output := ModImpl.output_sm ev in
-        let core0_output := ModImpl.output_core0 ev in
-        let core1_output := ModImpl.output_core1 ev in
-        match core_id with
-        | CoreId0 =>
-            {| obs_reqs := {| obs_imem_req := observe_imem_req0 (core0_output);
-                              obs_dmem_req := observe_dmem_req0 (core0_output)
-                           |};
-               obs_resps := {| obs_imem_resp := observe_imem_resp0 (sm_output);
-                               obs_dmem_resp := observe_dmem_resp0 (sm_output)
-                            |};
-               obs_encs := {| obs_enclave_req := observe_enclave_req0 (core0_output);
-                              obs_enclave_enter := observe_enclave_enter0 (sm_output);
-                              obs_enclave_exit := observe_enclave_exit0 (sm_output)
-                           |}
-            |}
-        | CoreId1 =>
-            {| obs_reqs := {| obs_imem_req := observe_imem_req1 (core1_output);
-                              obs_dmem_req := observe_dmem_req1 (core1_output)
-                           |};
-               obs_resps := {| obs_imem_resp := observe_imem_resp1 (sm_output);
-                               obs_dmem_resp := observe_dmem_resp1 (sm_output)
-                            |};
-               obs_encs := {| obs_enclave_req := observe_enclave_req1 (core1_output);
-                              obs_enclave_enter := observe_enclave_enter1 (sm_output);
-                              obs_enclave_exit := observe_enclave_exit1 (sm_output)
-                           |}
-           |}
-        end.
- *)
 
     (* TODO: might be easier to combine logs first *)
     Definition generate_observations__modSpec (ev: ModSpec.tau) : tau :=
@@ -1437,50 +1461,6 @@ Tactic Notation "destruct_vars" := destruct_vars_with auto.
         | CoreId0 => Spec.Machine0.do_observations log0 CoreId0
         | CoreId1 => Spec.Machine1.do_observations log1 CoreId1
          end.
-
-    (*
-      fun core_id =>
-        let sm0_output := fst (fst (ModSpec.output_sm ev)) in
-        let sm1_output := fst (snd (ModSpec.output_sm ev)) in
-        let core0_output := ModSpec.output_core0 ev in
-        let core1_output := ModSpec.output_core1 ev in
-        match core_id with
-        | CoreId0 =>
-            {| obs_reqs := {| obs_imem_req := observe_imem_req0 (core0_output);
-                              obs_dmem_req := observe_dmem_req0 (core0_output)
-                           |};
-               obs_resps := {| obs_imem_resp := observe_imem_resp0 (sm0_output);
-                               obs_dmem_resp := observe_dmem_resp0 (sm0_output)
-                            |};
-               obs_encs := {| obs_enclave_req := observe_enclave_req0 (core0_output);
-                              obs_enclave_enter := observe_enclave_enter0 (sm0_output);
-                              obs_enclave_exit := observe_enclave_exit0 (sm0_output)
-                           |}
-            |}
-        | CoreId1 =>
-            {| obs_reqs := {| obs_imem_req := observe_imem_req1 (core1_output);
-                              obs_dmem_req := observe_dmem_req1 (core1_output)
-                           |};
-               obs_resps := {| obs_imem_resp := observe_imem_resp1 (sm1_output);
-                               obs_dmem_resp := observe_dmem_resp1 (sm1_output)
-                            |};
-               obs_encs := {| obs_enclave_req := observe_enclave_req1 (core1_output);
-                              obs_enclave_enter := observe_enclave_enter1 (sm1_output);
-                              obs_enclave_exit := observe_enclave_exit1 (sm1_output)
-                           |}
-           |}
-        end.
-    *)
-
-    (* Ltac unfold_mod_impl_obs := *)
-    (*   unfold observe_imem_req0, observe_imem_req1, *)
-    (*          observe_dmem_req0, observe_dmem_req1, *)
-    (*          observe_imem_resp0, observe_imem_resp1, *)
-    (*          observe_dmem_resp0, observe_dmem_resp1, *)
-    (*          observe_enclave_req0, observe_enclave_req1, *)
-    (*          observe_enclave_enter0, observe_enclave_enter0, *)
-    (*          observe_enclave_exit0, observe_enclave_exit1 *)
-    (*          in *. *)
 
     (* TODO_MOVE *)
     Ltac unfold_impl_obs :=
@@ -1499,16 +1479,103 @@ Tactic Notation "destruct_vars" := destruct_vars_with auto.
     Import Observations.
     Import Interfaces.Common.
 
-    (* Inductive Sim (impl_st: ModImpl.state) (spec_st: ModSpec.state) := *)
-    (* | _Sim : *)
-    (*     forall (core0_sim: ModImpl.state_core0 impl_st = ModSpec.state_core0 spec_st), *)
-    (*     Sim impl_st spec_st. *)
-
     Section Simulation.
-      (* Lemma foo: *)
-      (*   forall (initial_dram: dram_t) (n: nat), *)
-      (*   snd (ModImpl.step_n_with_metadata initial_dram n) = *)
-      (*   snd (ModSpec.step_n_with_metadata initial_dram n). *)
+
+      Inductive Sim_step_io (impl_io: ModImpl.mod_step_io) (spec_io: ModSpec.mod_step_io) :=
+      | SimStepIo :
+          forall (core0_sim: impl_io.(ModImpl.step_io_core0) = spec_io.(ModSpec.step_io_core0))
+            (core1_sim: impl_io.(ModImpl.step_io_core1) = spec_io.(ModSpec.step_io_core1))
+            (sm_sim: impl_io.(ModImpl.step_io_sm) = fst (spec_io.(ModSpec.step_io_sm)))
+            (mem_sim: impl_io.(ModImpl.step_io_mem) = spec_io.(ModSpec.step_io_mem).(Mem_Common.ghost_step)),
+          Sim_step_io impl_io spec_io.
+
+      Ltac solve_forall_extract :=
+        apply Forall2_ind; auto; simpl; intros;
+        match goal with
+        | H: Sim_step_io _ _ |- _ => destruct H
+        end; rewrite_solve.
+
+      Property forall_sim_step_extract_core0 :
+        forall impl_ios spec_ios,
+        Forall2 Sim_step_io impl_ios spec_ios ->
+        map ModImpl.step_io_core0 impl_ios = map ModSpec.step_io_core0 spec_ios.
+      Proof.
+        solve_forall_extract.
+      Qed.
+
+      Property forall_sim_step_extract_core1 :
+        forall impl_ios spec_ios,
+        Forall2 Sim_step_io impl_ios spec_ios ->
+        map ModImpl.step_io_core1 impl_ios = map ModSpec.step_io_core1 spec_ios.
+      Proof.
+        solve_forall_extract.
+      Qed.
+
+      Property forall_sim_step_extract_sm :
+        forall impl_ios spec_ios,
+        Forall2 Sim_step_io impl_ios spec_ios ->
+        map ModImpl.step_io_sm impl_ios = map fst (map ModSpec.step_io_sm spec_ios).
+      Proof.
+        solve_forall_extract.
+      Qed.
+
+      Property forall_sim_step_extract_mem :
+        forall impl_ios spec_ios,
+        Forall2 Sim_step_io impl_ios spec_ios ->
+        map ModImpl.step_io_mem impl_ios = map Mem_Common.ghost_step (map ModSpec.step_io_mem spec_ios).
+      Proof.
+        solve_forall_extract.
+      Qed.
+
+      Definition core0_valid_input := @Core_Common.valid_input Core0.private_params.
+      Definition core0_valid_output := @Core_Common.valid_output Params0.core_id Params0.initial_pc Core0.private_params.
+      Definition core0_valid_feedback := @Core_Common.valid_feedback Params0.core_id Params0.initial_pc Core0.private_params.
+
+      Theorem step_n_ios_sim:
+        forall initial_dram n impl_st impl_tr spec_st spec_tr impl_io spec_io,
+        ModImpl.step_n_with_metadata initial_dram n = (impl_st, impl_tr, impl_io) ->
+        ModSpec.step_n_with_metadata initial_dram n = (spec_st, spec_tr, spec_io) ->
+        Forall2 Sim_step_io impl_io spec_io.
+      Proof.
+        induction n.
+        - intros; simpl in *; simplify_tupless; auto.
+        - intros *; intros HImpl HSpec.
+          specialize ModSpec.step_n_invariant with (1 := HSpec); intros HSpecInv; propositional.
+          simpl in HImpl, HSpec.
+          destruct_all_matches; simplify_tupless.
+          specialize IHn with (1 := eq_refl) (2 := eq_refl).
+          rename s1 into impl_st0; rename s into spec_st0.
+          rename m0 into impl_io; rename m into spec_io.
+
+          apply Forall2_app; auto.
+          constructor; auto.
+
+          (* Core0 valid input *)
+          assert (core0_valid_input spec_st0.(ModSpec.state_core0)
+                                    spec_io.(ModSpec.step_io_core0).(Core_Common.step_input))
+                 by admit.
+
+      Admitted.
+
+      Definition TODO_sm_trace_equivalent :=
+        @SM_Common.trace_equivalent Params0.initial_pc Params1.initial_pc
+                                    EnclaveParams.params External.ext.
+
+      Inductive GenTraceSim (impl_tr: ModImpl.trace) (spec_tr: ModSpec.trace) :=
+      | _SimTrace :
+          forall (core0_sim: (@Core_Common.trace_equivalent Core0.private_params)
+                          (map ModImpl.output_core0 impl_tr)
+                          (map ModSpec.output_core0 spec_tr))
+            (core1_sim: (@Core_Common.trace_equivalent Core1.private_params)
+                          (map ModImpl.output_core1 impl_tr)
+                          (map ModSpec.output_core1 spec_tr))
+            (sm_sim: TODO_sm_trace_equivalent
+                       (map ModImpl.output_sm impl_tr)
+                       (map ModSpec.output_sm spec_tr))
+            (mem_sim: (@Mem_Common.trace_equivalent Memory.private_params)
+                        (map ModImpl.output_mem impl_tr)
+                        (map ModSpec.output_mem spec_tr)),
+          GenTraceSim impl_tr spec_tr.
 
     End Simulation.
 
@@ -1519,6 +1586,21 @@ Tactic Notation "destruct_vars" := destruct_vars_with auto.
     Definition trace_related : ModImpl.trace -> ModSpec.trace -> Prop :=
       fun impl_tr spec_tr => List.Forall2 tau_related impl_tr spec_tr.
 
+    Lemma GenTraceSim_impl_trace_related :
+      forall impl_tr spec_tr,
+      GenTraceSim impl_tr spec_tr ->
+      trace_related impl_tr spec_tr.
+    Proof.
+    Admitted.
+
+    Ltac unfold_spec_props :=
+      consider ModSpec.valid_props;
+      consider ModSpec.valid_P_prop;
+      consider ModSpec.core0_P_prop;
+      consider ModSpec.core1_P_prop;
+      consider ModSpec.sm_P_prop;
+      consider ModSpec.mem_P_prop.
+
     Theorem refinement :
       forall (initial_dram: dram_t) (n: nat)
         (impl_st: ModImpl.state) (impl_tr: ModImpl.trace)
@@ -1527,37 +1609,48 @@ Tactic Notation "destruct_vars" := destruct_vars_with auto.
       ModSpec.step_n initial_dram n = (spec_st, spec_tr) ->
       trace_related impl_tr spec_tr.
     Proof.
-      intros.
-      consider trace_related.
-      consider tau_related.
-      consider ModImpl.trace.
-      consider ModSpec.trace.
+      intros *; intros HImplStep; intros HSpecStep.
+      apply ModImpl.step_n_extract_ios in HImplStep.
+      apply ModSpec.step_n_extract_ios in HSpecStep.
+      propositional.
+      specialize ModImpl.step_rel_decoupled_step__state with (1 := HImplStep0); intro HImplState.
+      specialize ModSpec.step_rel_decoupled_step__state with (1 := HSpecStep0); intro HSpecState.
+      specialize ModImpl.step_rel_decoupled_step__trace with (1 := HImplStep0); intro HImplTrace.
+      specialize ModSpec.step_rel_decoupled_step__trace with (1 := HSpecStep0); intro HSpecTrace.
+      apply GenTraceSim_impl_trace_related.
+      specialize step_n_ios_sim with (1 := HImplStep0) (2 := HSpecStep0); intros HSim.
+      specialize ModSpec.step_n_invariant with (1 := HSpecStep0); intros [HSpecInv HSpecProp]; propositional.
 
-
-
-      induction n.
-      - intros; simpl in *; simplify_tuples; subst; constructor.
-      - intros.
-        simpl in *
-
-
-
-
-simpl; intros.
-        destruct_all_matches; simplify_tuples; subst.
-        specialize IHn with (1 := eq_refl) (2 := eq_refl).
-        unfold trace_related.
-        apply Forall2_app; auto.
-        constructor; auto.
-
-        consider ModImpl.do_step.
-        destruct_all_matches.
-        (* consider ModSpec.do_step. *)
-        (* destruct_all_matches. *)
-        (* simplify_tuples. *)
-        (* subst. *)
-
-    Admitted.
+      constructor.
+      - specialize ModSpec.extract_core0_steps_from_metadata with (1 := HSpecStep0);
+        specialize ModImpl.extract_core0_steps_from_metadata with (1 := HImplStep0); intros.
+        propositional.
+        unfold_core0_steps.
+        rewrite forall_sim_step_extract_core0 with (1 := HSim) in *.
+        eapply Core0.correctness; eauto;
+          rewrite_term_from_tuple props; unfold_spec_props; intuition.
+      - specialize ModSpec.extract_core1_steps_from_metadata with (1 := HSpecStep0);
+        specialize ModImpl.extract_core1_steps_from_metadata with (1 := HImplStep0); intros.
+        propositional.
+        unfold_core1_steps.
+        rewrite forall_sim_step_extract_core1 with (1 := HSim) in *.
+        eapply Core1.correctness; eauto;
+          rewrite_term_from_tuple props; unfold_spec_props; intuition.
+      - specialize ModSpec.extract_sm_steps_from_metadata with (1 := HSpecStep0);
+        specialize ModImpl.extract_sm_steps_from_metadata with (1 := HImplStep0); intros.
+        propositional.
+        unfold_sm_steps.
+        rewrite forall_sim_step_extract_sm with (1 := HSim) in *.
+        eapply SM_Common.correctness; eauto;
+          rewrite_term_from_tuple props; unfold_spec_props; intuition.
+      - specialize ModSpec.extract_mem_steps_from_metadata with (1 := HSpecStep0);
+        specialize ModImpl.extract_mem_steps_from_metadata with (1 := HImplStep0); intros.
+        propositional.
+        unfold_mem_steps.
+        rewrite forall_sim_step_extract_mem with (1 := HSim) in *.
+        eapply Memory.correctness; eauto;
+          rewrite_term_from_tuple props; unfold_spec_props; intuition.
+    Qed.
 
   End ModImplToModSpec.
 
@@ -1612,8 +1705,8 @@ simpl; intros.
 
       Inductive GenTauSim (gen_ev: gen_impl_tau) (mod_ev: ModImpl.tau) :=
       | _GenTauSim :
-          forall (log_sim: fst gen_ev = ModImpl.outputs_to_impl_log mod_ev)
-            (mem_ext_st_sm : snd gen_ev = snd (ModImpl.output_mem mod_ev)),
+          forall (log_sim: fst gen_ev = ModImpl.outputs_to_impl_log mod_ev),
+            (* (mem_ext_st_sm : snd gen_ev = snd (ModImpl.output_mem mod_ev)), *)
           GenTauSim gen_ev mod_ev.
 
       Definition GenTraceSim (gen_tr: gen_impl_trace) (mod_tr: ModImpl.trace) : Prop :=
@@ -1941,7 +2034,7 @@ simpl; intros.
             auto_with_log_helpers.
           }
         }
-      Qed.
+      Admitted.
 
       Theorem step_n_sim :
         forall (initial_dram: dram_t) (n: nat)
@@ -2092,1333 +2185,4 @@ simpl; intros.
 
   End TopLevel.
 
-
-  (* ============== DEPRECATED ================== *)
 End TradPf.
-(*
-  Section Modularspec.
-    Record mod_step_tau_t :=
-      { mod_core0_output : Log Core0.R ContextEnv
-      ; mod_core1_output : Log Core1.R ContextEnv
-      ; sm_output__spec
-      }.
-
-  End ModularSpec.
-
-  Section Modular.
-    Record mod_step :=
-      { apres_core0: Log Impl.System.R ContextEnv;
-        apres_core1: Log Impl.System.R ContextEnv;
-        apres_sm   : Log Impl.System.R ContextEnv * sm_ghost_output_t;
-        final_log : Log Impl.System.R ContextEnv;
-        final_ext_state: Impl.placeholder_public_state
-      }.
-
-    (* TODO: (fancy?) notation *)
-    (* TODO:
-     * > Spec State
-     * > Modular spec state
-     * > Modular impl state
-     * > Impl
-     *)
-
-    (* TODO: generalize *)
-    Definition TODO_ghost_state_conversion (st: Impl.System.SM.ghost_output) : sm_ghost_output_t :=
-      {| ghost_output_config0 := Impl.System.SM.ghost_output_config0 st;
-         ghost_output_config1 := Impl.System.SM.ghost_output_config1 st
-      |}.
-
-    Definition do_core0_step (st: core0_state_t) (input_log: Log Impl.System.R ContextEnv)
-                             : Log Impl.System.R ContextEnv :=
-      let core0_log := proj_log (REnv := ContextEnv) Impl.System.Lift_core0 input_log in
-      let output_log := Core0.update_function st core0_log in
-      lift_log (REnv := ContextEnv) Impl.System.Lift_core0 output_log.
-
-    Definition do_core1_step (st: core1_state_t) (input_log: Log Impl.System.R ContextEnv)
-                             : Log Impl.System.R ContextEnv :=
-      let core1_log := proj_log (REnv := ContextEnv) Impl.System.Lift_core1 input_log in
-      let output_log := Core1.update_function st core1_log in
-      lift_log (REnv := ContextEnv) Impl.System.Lift_core1 output_log.
-
-    Definition do_sm_step (st: Impl.System.SM.state) (input_log: Log Impl.System.R ContextEnv)
-                          : Log Impl.System.R ContextEnv * sm_ghost_output_t :=
-      let sm_log := proj_log (REnv := ContextEnv) Impl.System.Lift_sm input_log in
-      let '(output_log, sm_ghost_output) := Impl.System.SM.update_function st sm_log in
-      (lift_log (REnv := ContextEnv) Impl.System.Lift_sm output_log, TODO_ghost_state_conversion sm_ghost_output).
-
-    Definition do_mem_step (st: Memory.state) (input_log: Log Impl.System.R ContextEnv)
-                          : Log Impl.System.R ContextEnv * Impl.placeholder_public_state :=
-      let mem_log := proj_log (REnv := ContextEnv) Impl.System.Lift_mem input_log in
-      let '(output_log, ext_st') := Memory.update_function st mem_log in
-      (lift_log (REnv' := ContextEnv) Impl.System.Lift_mem output_log, ext_st').
-
-    Definition get_mod_step__impl (impl_st: Impl.state) : mod_step :=
-      let koika_st := Impl.koika_state impl_st in
-      let apres_core0_log := do_core0_step (get_impl_core0 koika_st) log_empty in
-      let apres_core1_log := do_core1_step (get_impl_core1 koika_st) apres_core0_log in
-      (* SM *)
-      let sm_input := log_app apres_core1_log apres_core0_log in
-      let (apres_sm_log, sm_ghost_output) := do_sm_step (get_impl_sm koika_st) sm_input in
-      (* Mem *)
-      let mem_input := log_app apres_sm_log sm_input in
-      let (apres_mem_log, ext_st') := do_mem_step (get_impl_mem impl_st) mem_input in
-      let final := log_app apres_mem_log mem_input in
-      {| apres_core0 := apres_core0_log;
-         apres_core1 := apres_core1_log;
-         apres_sm := (apres_sm_log, sm_ghost_output);
-         final_log := final;
-         final_ext_state := ext_st'
-      |}.
-
-    Definition do_mod_step__impl (impl_st: Impl.state) (step: mod_step) : Impl.state :=
-      {| Impl.koika_state := commit_update (Impl.koika_state impl_st) (final_log step);
-         Impl.public_state := final_ext_state step
-      |}.
-
-    Fixpoint get_mod_steps__impl (initial_dram: dram_t) (n: nat) : Impl.state * list mod_step :=
-      match n with
-      | 0 => (Impl.initial_state initial_dram, [])
-      | S n' =>
-          let '(st, steps) := get_mod_steps__impl initial_dram n' in
-          let mod_step := get_mod_step__impl st in
-          (do_mod_step__impl st mod_step, steps ++ [mod_step])
-      end.
-
-    Definition mod_spec_st : Type. Admitted.
-    Definition mod_spec_tr : Type. Admitted.
-
-    Definition do_mod_steps__spec (initial_dram: dram_t) (steps: list mod_step)
-                                : mod_spec_st * mod_spec_tr.
-    Admitted.
-
-  End Modular.
-
-  (* TODO: this is just the standard layers. Can write as a framework later *)
-  Section ImplToModularImpl.
-
-    Definition impl_to_mod_impl_trace_equivalent : trace -> list mod_step -> Prop.
-    Admitted.
-
-    Lemma impl_to_mod_impl_refinement :
-      forall (initial_dram: dram_t) (n: nat)
-        (impl_st: Impl.state) (impl_tr: trace)
-        (mod_st: Impl.state) (mod_steps: list mod_step),
-        Impl.step_n initial_dram n = (impl_st, impl_tr) ->
-        get_mod_steps__impl initial_dram n = (mod_st, mod_steps) ->
-        impl_to_mod_impl_trace_equivalent impl_tr mod_steps.
-    Admitted.
-
-  End ImplToModularImpl.
-
-  Section ModularImplToModularSpec.
-    Definition mod_impl_to_mod_spec_trace_equivalent : list mod_step -> mod_spec_tr -> Prop.
-    Admitted.
-
-
-    Lemma mod_impl_to_mod_spec_refinement :
-      forall (initial_dram: dram_t) (n: nat)
-        (impl_st: Impl.state) (mod_steps: list mod_step)
-        (spec_st: mod_spec_st) (spec_tr: mod_spec_tr),
-        get_mod_steps__impl initial_dram n = (impl_st, mod_steps) ->
-        do_mod_steps__spec initial_dram mod_steps = (spec_st, spec_tr) ->
-        mod_impl_to_mod_spec_trace_equivalent mod_steps spec_tr.
-    Proof.
-    Admitted.
-
-  End ModularImplToModularSpec.
-
-  Section ModularSpecToSpec.
-    Lemma mod_spec_to_spec_refinement :
-      forall (initial_dram: dram_t) (n: nat)
-        (mod_st: mod_spec_st) (mod_tr: mod_spec_tr)
-        (spec_st: Spec.state) (spec_tr: trace),
-        ?get_mod_steps__impl initial_dram n = (impl_st, mod_steps) ->
-        Spec.step_n initial_dram n = (spec_st, spec_tr) ->
-
-
-  End ModularSpecToSpec.
-
-  Section Initialised.
-    Context (initial_dram : dram_t).
-
-    (* Proof idea:
-     * - reduce steps to input/output to individual modules, then use the modular proofs to do the lift
-     * - The modular proofs give us trace equivalence of the input/output effects of the impl and spec.
-     * - Need to show that impl_step_n <-> do_steps and similarly for spec
-     * - traces produced are the same implies we get trace equivalence!
-     *)
-    Lemma refinement': forall (n: nat)
-                          (impl_st: Impl.state) (impl_tr: trace)
-                          (spec_st: Spec.state) (spec_tr: trace),
-        Impl.step_n initial_dram n = (impl_st, impl_tr) ->
-        Spec.step_n initial_dram n = (spec_st, spec_tr) ->
-        impl_tr = spec_tr.
-    Proof.
-    Admitted.
-
-
-    Theorem refinement: forall (n: nat)
-                          (impl_st: Impl.state) (impl_tr: trace)
-                          (spec_st: Spec.state) (spec_tr: trace),
-        Impl.step_n initial_dram n = (impl_st, impl_tr) ->
-        Spec.step_n initial_dram n = (spec_st, spec_tr) ->
-        impl_tr = spec_tr.
-    Proof.
-
-
-
-
-
-
-(* ============================================================================ *)
-
-
-
-
-
-
-  Definition impl_state_t : Type := Impl.state * impl_ghost_state.
-  Definition spec_state_t : Type := Spec.state * spec_ghost_state.
-
-  Definition SpecInvariant0 (spec_core: @Spec.core_state_machine Spec.Machine0.state) : Prop :=
-    match spec_core with
-    | Spec.CoreState_Enclave _ _ _ => True (* TODO *)
-    | Spec.CoreState_Waiting new next_rf => True
-    end.
-
-  Definition SpecInvariant : spec_state_t -> Prop. Admitted.
-
-  (* TODO: very WIP; maybe an explicit ghost state will be better *)
-  Definition State0_Sim : Impl.state -> @Spec.core_state_machine Spec.Machine0.state -> Prop :=
-    fun '(impl_st, impl_ext) spec_core =>
-    match spec_core with
-    | Spec.CoreState_Enclave machine_state config enclave_state =>
-        (* Machine state simulation: *)
-        (* 1) Core0 is in the same state *)
-        get_impl_core0 impl_st = get_spec0_core0 machine_state /\
-        (* 2) Mem0 is in the same state, or we've had the same history of requests from a reset state?
-         *    Note: this might be better stated as a ghost-state property; TBD
-         *)
-        (* 3) SM? *)
-        (* enclave state *)
-        match enclave_state with
-        | Spec.EnclaveState_Running =>
-          True
-        | Spec.EnclaveState_Switching next => True
-        end
-    | Spec.CoreState_Waiting new next_rf =>
-        (* Core0 is in a reset state *)
-        Core0.valid_reset_state (get_impl_core0 impl_st) /\
-        (* Core0 is purged *)
-        ContextEnv.(getenv) impl_st impl_purge_mem0 = Common.ENUM_purge_purged /\
-        (* Mem0 is in a reset state *)
-        Memory.valid_reset_state (get_impl_mem impl_st) Common.CoreId0 /\
-        (* Mem0 is purged *)
-        ContextEnv.(getenv) impl_st impl_purge_mem0 = Common.ENUM_purge_purged /\
-        (* Rf is related *)
-        Impl.get_rf (impl_st,impl_ext) = next_rf /\
-        (* SM is in a certain state *)
-        SMProperties.valid_waiting_state (get_impl_sm impl_st) Common.CoreId0 new
-        (* TODO: Public memory is related *)
-    end.
-
-  Definition State1_Sim : Impl.state -> @Spec.core_state_machine Spec.Machine1.state -> Prop. Admitted.
-
-  Definition Clk_Sim : Impl.state -> bool -> Prop :=
-    fun '(impl_st, _) spec_clk =>
-      let impl_clk := getenv ContextEnv impl_st impl_sm_clk in
-      Bits.single impl_clk = spec_clk.
-
-  Definition StateSim : Impl.state -> Spec.state -> Prop :=
-    fun impl_st spec_st =>
-      State0_Sim impl_st (Spec.machine0_state spec_st) /\
-      State1_Sim impl_st (Spec.machine1_state spec_st) /\
-      Clk_Sim impl_st (Spec.clk spec_st).
-      (* TODO: Mem_Sim *)
-
-  Definition Sim (impl: impl_state_t) (spec: spec_state_t) : Prop :=
-    let (impl_st, impl_ghost) := impl in
-    let (spec_st, spec_ghost) := spec in
-    StateSim impl_st spec_st.
-
-  Section Initialised.
-    Variable initial_dram: dram_t.
-
-    Theorem initial_state_sim :
-      Sim (Impl.initial_state initial_dram, initial_impl_ghost)
-          (Spec.initial_state initial_dram, initial_spec_ghost).
-    Admitted.
-
-Ltac initialize :=
-  intros; unfold impl_state_t, spec_state_t in *; repeat destruct_pair.
-
-    Theorem step_sim : forall (impl_st impl_st': impl_state_t) (spec_st spec_st': spec_state_t)
-                         (impl_tau spec_tau: tau),
-      Sim impl_st spec_st ->
-      impl_step_with_ghost impl_st = (impl_st', impl_tau) ->
-      spec_step_with_ghost spec_st = (spec_st', spec_tau) ->
-      Sim impl_st' spec_st' /\ impl_tau = spec_tau.
-    Proof.
-      initialize.
-      unfold impl_step_with_ghost, Impl.step in *.
-      unfold spec_step_with_ghost, Spec.step in *.
-      destruct_all_matches.
-      simplify_all.
-
-      unfold Impl.do_observations.
-      unfold Spec.do_magic_step in Heqp.
-      destruct_outer_match_in_hyp Heqp; simplify_tuples; subst.
-
-      { (* Case1: MagicState_Continue *)
-        unfold Spec.local_core_step in Heqm1.
-        destruct_outer_match_in_hyp Heqm1.
-        { (* Case: Spec.CoreState_Enclave *)
-          destruct_outer_match_in_hyp Heqm1.
-          (* TODO: Machine step invariant: show preservation *)
-          destruct_outer_match_in_hyp Heqm1.
-          { (* Case: Spec.EnclaveState_Running *)
-            (* Invariant preservation, log preservation *)
-            admit.
-          }
-          { destruct_ite_in_hyp Heqm1; try congruence.
-            (* Case: Spec.EnclaveState_Switching; no exit *)
-            inversion_clear Heqm1.
-            (* Invariant preservation *)
-          admit.
-          }
-        }
-        { destruct_ite_in_hyp Heqm1; try congruence.
-          (* Case: Spec.CoreState_Waiting; no switch *)
-          inversion_clear Heqm1.
-          (* Idea: Spec.clk spec_st0 = true ->
-             Core0 still in reset and Mem0 still in reset *)
-          (* Therefore no update to logs, therefore empty observations *)
-          admit.
-        }
-      }
-      { (* Case2: Spec.MagicState_Exit *)
-        unfold Spec.local_core_step in Heqm1.
-        repeat destruct_matches_in_hyp Heqm1; try congruence.
-        inversion_clear Heqm1.
-        (* Idea: Simulation in terms of SM; prove that Impl step exits too *)
-        admit.
-      }
-      { (* Case3: Spec.MagicState_Enter *)
-        destruct_ite_in_hyp Heqp.
-        { (* Case: Spec.can_enter *)
-          simplify_all.
-          (* Initial enclave simulation: Impl enters enclave too *)
-          admit.
-        }
-        { (* Case: Spec can not enter; no change *)
-          simplify_all.
-          admit.
-        }
-      }
-    Admitted.
-
-    Theorem step_n_sim : forall (n: nat)
-                         (impl_st: Impl.state) (impl_tr: trace) (impl_ghost: impl_ghost_state)
-                         (spec_st: Spec.state) (spec_tr: trace) (spec_ghost: spec_ghost_state),
-        impl_step_n_with_ghost initial_dram n = ((impl_st, impl_ghost), impl_tr) ->
-        spec_step_n_with_ghost initial_dram n = ((spec_st, spec_ghost), spec_tr) ->
-        Sim (impl_st, impl_ghost) (spec_st, spec_ghost) /\ impl_tr = spec_tr.
-    Proof.
-      induction n.
-      - intros; simplify_all; split_cases; auto.
-        apply initial_state_sim.
-      - simpl; intros; destruct_all_matches; simplify_all.
-        repeat destruct_pair.
-        specialize IHn with (1 := eq_refl) (2 := eq_refl); propositional.
-        match goal with
-        | [ H0: Sim _ _,
-            H1: impl_step_with_ghost _ = _,
-            H2: spec_step_with_ghost _ = _ |- _ ] =>
-          specialize step_sim with (1 := H0) (2 := H1) (3 := H2)
-        end.
-        intuition.
-    Qed.
-
-    Theorem refinement: forall (n: nat)
-                          (impl_st: Impl.state) (impl_tr: trace)
-                          (spec_st: Spec.state) (spec_tr: trace),
-        Impl.step_n initial_dram n = (impl_st, impl_tr) ->
-        Spec.step_n initial_dram n = (spec_st, spec_tr) ->
-        impl_tr = spec_tr.
-    Proof.
-      intros *; intros H_impl H_spec.
-      destruct (impl_step_n_with_ghost initial_dram n) as [[impl_st' impl_ghost] impl_tr'] eqn:Heq_impl.
-      destruct (spec_step_n_with_ghost initial_dram n) as [[spec_st' spec_ghost] spec_tr'] eqn:Heq_spec.
-      edestruct impl_drop_ghost with (1 := Heq_impl) (2 := H_impl).
-      edestruct spec_drop_ghost with (1 := Heq_spec) (2 := H_spec).
-      simplify_all.
-      eapply step_n_sim; eauto.
-    Qed.
-
-  End Initialised.
-
-End TradPf.
-
-(* DEPRECATED *)
-(*
-  Module SMProperties.
-    Include Interfaces.Common.
-    Include Interfaces.EnclaveInterface.
-    Include Impl.System.SM.
-
-    Section Semantics.
-      Definition empty_log : Log R ContextEnv := log_empty.
-      Parameter update_function : state -> Log R ContextEnv -> Log R ContextEnv.
-        (* Except without the append *)
-        (* interp_scheduler' st ? rules log scheduler. *)
-
-      (* Output intermediate log *)
-      Definition step (st: state) (input: Log R ContextEnv) (feedback: Log R ContextEnv)
-                      : state * Log R ContextEnv :=
-        let output := update_function st input in
-        (commit_update st (log_app feedback (log_app output input)), output).
-
-    End Semantics.
-
-    Section LogHelpers.
-      Definition update_no_writes_to_reg (st: state) (log: Log R ContextEnv) (reg: reg_t) : Prop :=
-        latest_write (update_function st log) reg = latest_write log reg.
-
-    End LogHelpers.
-
-    Import EnclaveInterface.
-
-    Section IsolatedSystem.
-
-      Inductive enclave_state_t :=
-      | EnclaveState_Running
-      | EnclaveState_Switching (next_enclave: enclave_config)
-      .
-
-      Inductive sm_state_machine :=
-      | SmState_Enclave (machine_state: state) (config: enclave_config)
-                        (enclave_state: enclave_state_t)
-      | SmState_Waiting (new: enclave_config).
-
-      Inductive sm_magic_state_machine :=
-      | SmMagicState_Continue (st: sm_state_machine) (ext: Log R ContextEnv)
-      | SmMagicState_Exit (waiting: enclave_config) (ext: Log R ContextEnv)
-      | SmMagicState_TryToEnter (next_enclave: enclave_config).
-
-      Record iso_machine_t :=
-        { iso_sm0 : sm_state_machine;
-          iso_sm1 : sm_state_machine;
-          turn : bool
-        }.
-
-      Inductive taint_t :=
-      | TaintCore (core_id: ind_core_id)
-      | Bottom.
-
-      Definition private_reg_to_taint (reg: private_reg_t) : taint_t :=
-        match reg with
-        | state0 => TaintCore CoreId0
-        | state1 => TaintCore CoreId1
-        | enc_data0 => TaintCore CoreId0
-        | enc_data1 => TaintCore CoreId1
-        | enc_req0 => TaintCore CoreId0
-        | enc_req1 => TaintCore CoreId1
-        | clk => Bottom
-        end.
-
-      Definition reg_to_taint (reg: reg_t) : taint_t :=
-        match reg with
-        | fromCore0_IMem st => TaintCore CoreId0
-        | fromCore0_DMem st => TaintCore CoreId0
-        | fromCore0_Enc st => TaintCore CoreId0
-        | toCore0_IMem st => TaintCore CoreId0
-        | toCore0_DMem st => TaintCore CoreId0
-        (* Core1 <-> SM *)
-        | fromCore1_IMem st => TaintCore CoreId1
-        | fromCore1_DMem st => TaintCore CoreId1
-        | fromCore1_Enc st => TaintCore CoreId1
-        | toCore1_IMem st => TaintCore CoreId1
-        | toCore1_DMem st => TaintCore CoreId1
-        (* SM <-> Mem *)
-        | toMem0_IMem st => TaintCore CoreId0
-        | toMem0_DMem st => TaintCore CoreId0
-        | toMem1_IMem st => TaintCore CoreId1
-        | toMem1_DMem st => TaintCore CoreId1
-        | fromMem0_IMem st => TaintCore CoreId0
-        | fromMem0_DMem st => TaintCore CoreId0
-        | fromMem1_IMem st => TaintCore CoreId1
-        | fromMem1_DMem st => TaintCore CoreId1
-        | pc_core0 => TaintCore CoreId0
-        | pc_core1 => TaintCore CoreId1
-        | purge_core0 => TaintCore CoreId0
-        | purge_core1 => TaintCore CoreId1
-        | purge_mem0 => TaintCore CoreId0
-        | purge_mem1 => TaintCore CoreId1
-        | private st => private_reg_to_taint st
-      end.
-
-      Scheme Equality for taint_t.
-
-      Definition filter_public (log: Log R ContextEnv) (core: ind_core_id) : Log R ContextEnv :=
-        ContextEnv.(create) (fun r => match r with
-                                   | private s => []
-                                   | reg => if (taint_t_beq (reg_to_taint reg) (TaintCore core))
-                                              || (taint_t_beq (reg_to_taint reg) Bottom) then
-                                              ContextEnv.(getenv) log reg
-                                           else []
-                                   end).
-
-      Definition check_for_context_switching (core_id: ind_core_id) (input_log: Log R ContextEnv)
-                                             : option EnclaveInterface.enclave_config.
-      Admitted.
-
-      Definition bits_eqb {sz} (v1: bits_t sz) (v2: bits_t sz) : bool :=
-        N.eqb (Bits.to_N v1) (Bits.to_N v2).
-
-      (* TODO: normal way of writing this? *)
-      Definition observe_enclave_exit (core_id: ind_core_id) (log: Log R ContextEnv) : bool.
-        refine(
-        let enc_data_reg := match core_id with
-                            | CoreId0 => private enc_data0
-                            | CoreId1 => private enc_data1
-                            end in
-        match rew_latest_write log enc_data_reg _ with
-        | Some v =>
-            let data := EnclaveInterface.extract_enclave_data v in
-            bits_eqb (EnclaveInterface.enclave_data_valid data) Ob~0
-        | None => false
-        end).
-        - destruct core_id; reflexivity.
-      Defined.
-
-      Definition local_core_step (can_switch: bool) (core_id: ind_core_id)
-                                 (config: sm_state_machine) (input: Log R ContextEnv) (feedback: Log R ContextEnv)
-                                 : sm_magic_state_machine * Prop * Prop :=
-        let TODO_valid_input := True in
-        let TODO_valid_feedback := True in
-        let st :=
-          match config with
-          | SmState_Enclave machine enclave enclave_state =>
-              let (machine', output_log) := step machine input feedback in
-              (* let output_log := filter_public *)
-              match enclave_state with
-              | EnclaveState_Running =>
-                  let enclave_state' :=
-                    match check_for_context_switching core_id input with
-                    | Some next_enclave => EnclaveState_Switching next_enclave
-                    | None => EnclaveState_Running
-                    end in
-                  SmMagicState_Continue (SmState_Enclave machine' enclave enclave_state') output_log
-              | EnclaveState_Switching next_enclave =>
-                  if observe_enclave_exit core_id output_log
-                  then SmMagicState_Exit next_enclave output_log
-                  else SmMagicState_Continue (SmState_Enclave machine' enclave enclave_state) output_log
-              end
-          | SmState_Waiting next_enclave =>
-              if can_switch
-              then SmMagicState_TryToEnter next_enclave
-              else SmMagicState_Continue config empty_log
-          end in
-        (st, TODO_valid_input, TODO_valid_feedback).
-
-      Definition can_enter_enclave (next_enclave: enclave_config) (other_core_enclave: option enclave_config) : bool :=
-        match other_core_enclave with
-        | None => true
-        | Some config =>
-            (* Other core hasn't claimed the requested memory regions *)
-            negb (enclave_id_beq next_enclave.(eid) config.(eid)) &&
-            negb (next_enclave.(shared_page) && config.(shared_page))
-        end.
-
-      Definition enclave_config_to_enclave_data (config: enclave_config) : struct_t enclave_data :=
-        mk_enclave_data {| enclave_data_eid := enclave_id_to_bits config.(eid);
-                           enclave_data_addr_min := EnclaveParams.enclave_base config.(eid);
-                           enclave_data_size := EnclaveParams.enclave_size config.(eid);
-                           enclave_data_shared_page := if config.(shared_page) then Ob~1 else Ob~0;
-                           enclave_data_valid := Ob~1
-                        |}.
-
-      Definition TODO_spin_up_machine (core: ind_core_id) (next: enclave_config) (turn: bool) : state :=
-        ContextEnv.(create) (fun reg => match reg return R reg with
-                                   | private enc_data0 =>
-                                       if ind_core_id_beq core CoreId0
-                                       then enclave_config_to_enclave_data next
-                                       else r (private enc_data0)
-                                   | private enc_data1 =>
-                                       if ind_core_id_beq core CoreId1
-                                       then enclave_config_to_enclave_data next
-                                       else r (private enc_data1)
-                                   | private clk => if turn then Ob~1 else Ob~0
-                                   | reg' => r reg'
-                                   end).
-
-      Definition do_magic_step (core: ind_core_id)
-                               (turn: bool)
-                               (config: sm_magic_state_machine)
-                               (other_cores_enclave: option enclave_config)
-                               : sm_state_machine * Log R ContextEnv :=
-        match config with
-        | SmMagicState_Continue st obs => (st, obs)
-        | SmMagicState_Exit next_enclave obs =>
-           (SmState_Waiting next_enclave, obs)
-        | SmMagicState_TryToEnter next_enclave =>
-            if can_enter_enclave next_enclave other_cores_enclave then
-              let machine := TODO_spin_up_machine core next_enclave turn in
-              let sm_state := SmState_Enclave machine next_enclave EnclaveState_Running in
-              let obs := empty_log in (* TODO *)
-              (sm_state, obs)
-             else (SmState_Waiting next_enclave, empty_log)
-        end.
-
-      Definition get_enclave_config (st: sm_state_machine) : option enclave_config :=
-        match st with
-        | SmState_Enclave _ config _ => Some config
-        | _ => None
-        end.
-
-      Definition iso_step (st: iso_machine_t) (input: Log R ContextEnv) (feedback: Log R ContextEnv)
-                          : iso_machine_t * (Log R ContextEnv * Log R ContextEnv) :=
-        let magic0 := local_core_step (negb st.(turn)) CoreId0 st.(iso_sm0)
-                                      (filter_public input CoreId0) (filter_public feedback CoreId0) in
-        let magic1 := local_core_step st.(turn) CoreId1 st.(iso_sm1)
-                                      (filter_public input CoreId1) (filter_public feedback CoreId1) in
-        let '(iso0', log0) := do_magic_step CoreId0 (negb st.(turn)) magic0 (get_enclave_config st.(iso_sm1)) in
-        let '(iso1', log1) := do_magic_step CoreId1 (negb st.(turn)) magic1 (get_enclave_config st.(iso_sm0)) in
-        let st' := {| iso_sm0 := iso0';
-                      iso_sm1 := iso1';
-                      turn := negb st.(turn)
-                   |} in
-        (st', (log0, log1)). (* TODO: process log0 and log1 *)
-
-    End IsolatedSystem.
-
-    Section ValidInput.
-      (* Input log is valid iff
-       * - only touches interface/public registers
-       * - only enqueues/dequeues to relevant FIFOs
-       * - any write to purge_core is well-behaved as per purge state machine model
-       *)
-      (* Feedback log is similarly valid as above. Not very interesting *)
-      (* Valid output is a function of state:
-       * - We want to say the output addresses belong to disjoint taints in a sense, but we can derive this.
-       * - Also enough to say that the outputs belong to the enclave,
-       *)
-
-      Definition valid_input_log (st: state) (log: Log R ContextEnv) : Prop. Admitted.
-      Definition valid_input_state (st: state) : Prop. Admitted.
-      Definition valid_feedback_log : state -> Log R ContextEnv -> Log R ContextEnv -> Prop. Admitted.
-    End ValidInput.
-
-    Section Correctness.
-      Theorem correctness:
-
-
-    End Correctness.
-
-    Section Compliance.
-
-    End Compliance.
-
-
-      Inductive taint_t :=
-      | TaintCore (core_id: ind_core_id)
-      | Bottom.
-
-      (* More generic framework:
-       * time partition based on contents of a register, which is deterministic.
-       * So function from time to taint.
-       * Idea is that equivalence holds as an independent function of time?;
-       * Note: SM is entirely spatially partitioned. Normally this would need to be a function of time too
-       *)
-      Definition private_reg_to_taint (reg: private_reg_t) : taint_t :=
-        match reg with
-        | state0 => TaintCore CoreId0
-        | state1 => TaintCore CoreId1
-        | enc_data0 => TaintCore CoreId0
-        | enc_data1 => TaintCore CoreId1
-        | enc_req0 => TaintCore CoreId0
-        | enc_req1 => TaintCore CoreId1
-        | clk => Bottom
-        end.
-
-      Definition reg_to_taint (reg: reg_t) : taint_t :=
-        match reg with
-        | fromCore0_IMem st => TaintCore CoreId0
-        | fromCore0_DMem st => TaintCore CoreId0
-        | fromCore0_Enc st => TaintCore CoreId0
-        | toCore0_IMem st => TaintCore CoreId0
-        | toCore0_DMem st => TaintCore CoreId0
-        (* Core1 <-> SM *)
-        | fromCore1_IMem st => TaintCore CoreId1
-        | fromCore1_DMem st => TaintCore CoreId1
-        | fromCore1_Enc st => TaintCore CoreId1
-        | toCore1_IMem st => TaintCore CoreId1
-        | toCore1_DMem st => TaintCore CoreId1
-        (* SM <-> Mem *)
-        | toMem0_IMem st => TaintCore CoreId0
-        | toMem0_DMem st => TaintCore CoreId0
-        | toMem1_IMem st => TaintCore CoreId1
-        | toMem1_DMem st => TaintCore CoreId1
-        | fromMem0_IMem st => TaintCore CoreId0
-        | fromMem0_DMem st => TaintCore CoreId0
-        | fromMem1_IMem st => TaintCore CoreId1
-        | fromMem1_DMem st => TaintCore CoreId1
-        | pc_core0 => TaintCore CoreId0
-        | pc_core1 => TaintCore CoreId1
-        | purge_core0 => TaintCore CoreId0
-        | purge_core1 => TaintCore CoreId1
-        | purge_mem0 => TaintCore CoreId0
-        | purge_mem1 => TaintCore CoreId1
-        | private st => private_reg_to_taint st
-      end.
-
-    End ValidInput.
-
-    Section Initialise.
-
-      Definition private_waiting_state (eid_req0: option enclave_id) (eid_req1: option enclave_id)
-                                        (clk: bits_t 1) (idx: private_reg_t) : R_private idx :=
-        match idx with
-        | state0 => ENUM_CORESTATE_WAITING
-        | state1 => ENUM_CORESTATE_WAITING
-        | enc_data0 => value_of_bits (Bits.zero)
-        | enc_data1 => value_of_bits (Bits.zero)
-        | enc_req0 =>
-           match eid_req0 with
-           | Some id => eid_to_initial_enclave_data id
-           | None => value_of_bits Bits.zero
-           end
-        | enc_req1 =>
-           match eid_req1 with
-           | Some id => eid_to_initial_enclave_data id
-           | None => value_of_bits Bits.zero
-           end
-        | clk => clk
-        end.
-
-      Definition initialise_private_with_eid
-                 (eid0: option enclave_id) (eid1: option enclave_id) (clk: bits_t 1)
-                 (idx: private_reg_t) : R_private idx :=
-        match idx with
-        | state0 => value_of_bits Bits.zero
-        | state1 => value_of_bits Bits.zero
-        | enc_data0 =>
-           match eid0 with
-           | Some id => eid_to_initial_enclave_data id
-           | None => value_of_bits (Bits.zero)
-           end
-        | enc_data1 =>
-           match eid1 with
-           | Some id => eid_to_initial_enclave_data id
-           | None => value_of_bits (Bits.zero)
-           end
-        | enc_req0 => value_of_bits (Bits.zero)
-        | enc_req1 => value_of_bits (Bits.zero)
-        | clk => clk
-        end.
-
-      Definition initialise_waiting_r (eid_req0: option enclave_id) (eid_req1: option enclave_id)
-                                      (clk: bits_t 1) (idx: reg_t) : R idx :=
-        match idx with
-        | private s => private_waiting_state eid_req0 eid_req1 clk s
-        | s => r s
-        end.
-
-      Definition initialise_with_eid (eid0: option enclave_id) (eid1: option enclave_id)
-                                     (clk: bits_t 1) (idx: reg_t) : R idx :=
-        match idx with
-        | private s => initialise_private_with_eid eid0 eid1 clk s
-        | s => r s
-        end.
-
-    End Initialise.
-
-    Section ValidResetState.
-      (* TODO: clk ignored *)
-      Definition valid_waiting_state (st: state) (core_id: ind_core_id)
-                                     (next: EnclaveInterface.enclave_config) : Prop :=
-        forall reg, reg_to_taint reg = TaintCore core_id ->
-               (reg <> pc_core0 /\ reg <> pc_core1) ->
-               match core_id with
-               | CoreId0 => initialise_waiting_r (Some next.(EnclaveInterface.eid)) None Ob~0 reg
-                           = ContextEnv.(getenv) st reg
-               | CoreId1 => initialise_waiting_r None (Some next.(EnclaveInterface.eid)) Ob~0 reg
-                           = ContextEnv.(getenv) st reg
-               end.
-
-      (* TODO: not quite complete. *)
-      Definition valid_reset_state (st: state) (core_id: ind_core_id) (eid: enclave_id): Prop :=
-        forall reg, reg_to_taint reg = TaintCore core_id ->
-               (reg <> pc_core0 /\ reg <> pc_core1) ->
-               match core_id with
-               | CoreId0 => initialise_with_eid (Some eid) None Ob~0 reg = ContextEnv.(getenv) st reg
-               | CoreId1 => initialise_with_eid None (Some eid) Ob~0 reg = ContextEnv.(getenv) st reg
-               end.
-
-    End ValidResetState.
-
-    Section SMPrivateAxioms.
-
-      Definition valid_enclave_data (data: struct_t enclave_data) : Prop :=
-        let enclave_data := extract_enclave_data data in
-        match bits_id_to_ind_id enclave_data.(enclave_data_eid) with
-        | Some id =>
-            enclave_data.(enclave_data_addr_min) = EnclaveParams.enclave_base id /\
-            enclave_data.(enclave_data_size) = EnclaveParams.enclave_size id
-        | None => False
-        end.
-
-      Definition valid_enclave_data_regs (st: state) : Prop :=
-        valid_enclave_data (ContextEnv.(getenv) st (private enc_data0)) /\
-        valid_enclave_data (ContextEnv.(getenv) st (private enc_data1)).
-
-      (* TODO: incomplete *)
-      Definition valid_private_state (st: state) : Prop :=
-        valid_enclave_data_regs st.
-
-      Definition state_eq (st: state) (core_id: ind_core_id) (v: enum_t core_state): Prop :=
-        match core_id with
-        | CoreId0 => ContextEnv.(getenv) st (private state0) = v
-        | CoreId1 => ContextEnv.(getenv) st (private state1) = v
-        end.
-
-      (* Idea:
-       * - ghost state tracks when cores are done purging and when cores have restarted?
-       * - or we explicitly add it to the observations! <-- This seems better, since it defines what we care about
-       *)
-
-      Definition equiv_log_at_core (core_id: ind_core_id) (log1: Log R ContextEnv) (log2: Log R ContextEnv) : Prop :=
-        forall r, reg_to_taint r = TaintCore core_id ->
-             ContextEnv.(getenv) log1 r = ContextEnv.(getenv) log2 r.
-
-      Definition equiv_log_at_shared (log1: Log R ContextEnv) (log2: Log R ContextEnv) : Prop :=
-        forall r, reg_to_taint r = Bottom ->
-             ContextEnv.(getenv) log1 r = ContextEnv.(getenv) log2 r.
-
-      Definition equiv_log_for_core (core_id: ind_core_id) (log1: Log R ContextEnv) (log2: Log R ContextEnv) : Prop :=
-        equiv_log_at_core core_id log1 log2 /\ equiv_log_at_shared log1 log2.
-
-      Definition equiv_st_at_core (core_id: ind_core_id) (st1: state) (st2: state) : Prop :=
-        forall r, reg_to_taint r = TaintCore core_id ->
-             ContextEnv.(getenv) st1 r = ContextEnv.(getenv) st2 r.
-
-      Definition equiv_st_at_shared (st1: state) (st2: state) : Prop :=
-        forall r, reg_to_taint r = Bottom ->
-             ContextEnv.(getenv) st1 r = ContextEnv.(getenv) st2 r.
-
-      Definition equiv_st_for_core (core_id: ind_core_id) (st1: state) (st2: state) : Prop :=
-        equiv_st_at_core core_id st1 st2 /\ equiv_st_at_shared st1 st2.
-
-      (* Assuming we are not initially in a limbo state, output is a function only of taint0 registers *)
-      Definition output_is_a_function_of_partitioned_registers:
-        forall (core_id: ind_core_id) (st0 st1: state) (log0 log1: Log R ContextEnv),
-        state_eq st0 core_id (value_of_bits Bits.zero) ->
-        valid_input_state st0 ->
-        valid_input_state st1 ->
-        valid_input_log st0 log0 ->
-        valid_input_log st1 log1 ->
-        equiv_st_for_core core_id st0 st1 ->
-        equiv_log_for_core core_id log0 log1 ->
-        equiv_log_for_core core_id (update_function st0 log0) (update_function st1 log1).
-      Admitted.
-
-      (* TODO: figure out dependent types *)
-      Definition no_enq_to_output_reg (core_id: ind_core_id) (reg: reg_t) (log: Log R ContextEnv): Prop :=
-        match reg with
-        | toCore0_IMem MemResp.valid0 =>
-            core_id = CoreId0 /\
-            latest_write log (toCore0_IMem MemResp.valid0) <> Some Ob~1
-        | toCore0_DMem MemResp.valid0 =>
-            core_id = CoreId0 /\
-            latest_write log (toCore0_DMem MemResp.valid0) <> Some Ob~1
-        | toMem0_IMem MemReq.valid0 =>
-            core_id = CoreId0 /\
-            latest_write log (toMem0_IMem MemReq.valid0) <> Some Ob~1
-        | toMem0_DMem MemReq.valid0 =>
-            core_id = CoreId0 /\
-            latest_write log (toMem0_DMem MemReq.valid0) <> Some Ob~1
-        | toCore1_IMem MemResp.valid0 =>
-            core_id = CoreId1 /\
-            latest_write log (toCore1_IMem MemResp.valid0) <> Some Ob~1
-        | toCore1_DMem MemResp.valid0 =>
-            core_id = CoreId1 /\
-            latest_write log (toCore1_DMem MemResp.valid0) <> Some Ob~1
-        | toMem1_IMem MemReq.valid0 =>
-            core_id = CoreId1 /\
-            latest_write log (toMem1_IMem MemReq.valid0) <> Some Ob~1
-        | toMem1_DMem MemReq.valid0 =>
-            core_id = CoreId1 /\
-            latest_write log (toMem1_DMem MemReq.valid0) <> Some Ob~1
-        | _ => False
-        end.
-
-      (* TODO: rephrase this. This is annoying to work with *)
-      Definition no_public_enqs (core_id: ind_core_id) (st: state) (log: Log R ContextEnv) : Prop :=
-        forall reg, no_enq_to_output_reg core_id reg (update_function st log) \/
-               update_no_writes_to_reg st log reg.
-
-    End SMPrivateAxioms.
-
-    (* TODO: this needs to be in a framework *)
-    Section CycleModel.
-      Record step_params :=
-        { param_input : Log R ContextEnv;
-          param_feedback: Log R ContextEnv -> Log R ContextEnv
-        }.
-
-      Definition prop_holds_about_sm_step (st: state) (params: step_params)
-                                          (P: state -> Log R ContextEnv -> Log R ContextEnv -> Log R ContextEnv -> Prop) : Prop :=
-        let update := update_function st params.(param_input) in
-        let final := params.(param_feedback) update in
-        P st params.(param_input) update final.
-
-      (* Given a valid input state and input log, for any state' log' that are related,
-       * the output log is the same.
-       *)
-      Definition P_partition (core_id: ind_core_id)
-                 (st: state) (input_log output_log feedback_log: Log R ContextEnv) : Prop :=
-        forall st' log',
-        (*
-        valid_input_state st' ->
-        valid_input_log st log' ->
-        *)
-        equiv_st_for_core core_id st st' ->
-        equiv_log_for_core core_id input_log log' ->
-        equiv_log_for_core core_id output_log (update_function st' log').
-
-      Definition do_step (st: state) (input_log: Log R ContextEnv)
-                         (feedback_fn: Log R ContextEnv -> Log R ContextEnv) :=
-        let update := update_function st input_log in
-        let final := feedback_fn update in
-        commit_update st final.
-
-      (* Model cycle with input, schedule, post-schedule update
-       * Important points
-       * - From a reset state, requests to memory are a function only of inputs to relevant core,
-       *   until a context switch is requested
-       * - All requests to memory are within range of the enclave
-       * - When a context switch is requested, we have no more requests to memory
-       * - Need something about how the time it takes for memory/core to reset is independent...,
-       *   but that's not here
-       *)
-
-      (* TODO: restructure *)
-      Definition observe_enclave_reqs (log: Log R ContextEnv) (core_id: ind_core_id) : option (struct_t enclave_req).
-      Admitted.
-
-      Definition valid_enclave_req (req: struct_t enclave_req) : Prop :=
-        let '(eid, _) := req in
-        Bits.to_nat eid < 4.
-
-      Definition P_no_enclave_req (core_id: ind_core_id)
-                                  : state -> Log R ContextEnv -> Log R ContextEnv -> Log R ContextEnv -> Prop :=
-        fun st input_log output_log _ =>
-          match observe_enclave_reqs output_log core_id with
-          | None => True
-          | Some req => not (valid_enclave_req req)
-          end.
-
-      Definition observe_imem_reqs_to_mem0 (log: Log R ContextEnv) : option (struct_t mem_req) :=
-        observe_enq0 (toMem0_IMem MemReq.valid0) eq_refl
-                     (toMem0_IMem MemReq.data0) eq_refl
-                     log.
-
-      Definition observe_imem_reqs_to_mem1 (log: Log R ContextEnv) : option (struct_t mem_req) :=
-        observe_enq0 (toMem1_IMem MemReq.valid0) eq_refl
-                     (toMem1_IMem MemReq.data0) eq_refl
-                     log.
-
-      Definition observe_imem_reqs_to_mem (log: Log R ContextEnv) (core_id: ind_core_id) : option (struct_t mem_req) :=
-        match core_id with
-        | CoreId0 => observe_imem_reqs_to_mem0 log
-        | CoreId1 => observe_imem_reqs_to_mem1 log
-        end.
-
-      Definition observe_dmem_reqs_to_mem0 (log: Log R ContextEnv) : option (struct_t mem_req) :=
-        observe_enq0 (toMem0_DMem MemReq.valid0) eq_refl
-                     (toMem0_DMem MemReq.data0) eq_refl
-                     log.
-
-      Definition observe_dmem_reqs_to_mem1 (log: Log R ContextEnv) : option (struct_t mem_req) :=
-        observe_enq0 (toMem1_DMem MemReq.valid0) eq_refl
-                     (toMem1_DMem MemReq.data0) eq_refl
-                     log.
-
-      Definition observe_dmem_reqs_to_mem (log: Log R ContextEnv) (core_id: ind_core_id) : option (struct_t mem_req) :=
-        match core_id with
-        | CoreId0 => observe_dmem_reqs_to_mem0 log
-        | CoreId1 => observe_dmem_reqs_to_mem1 log
-        end.
-
-      Definition P_mem_reqs_in_range (mem: ind_cache_type) (core_id: ind_core_id) (eid: enclave_id)
-                                     : state -> Log R ContextEnv -> Log R ContextEnv -> Log R ContextEnv -> Prop :=
-        let addr_min := EnclaveParams.enclave_base eid in
-        let addr_max := Bits.plus (EnclaveParams.enclave_base eid) (EnclaveParams.enclave_size eid) in
-        fun st input_log output_log _ =>
-          let req_opt := match mem with
-                         | CacheType_Imem => observe_imem_reqs_to_mem output_log core_id
-                         | CacheType_Dmem => observe_dmem_reqs_to_mem output_log core_id
-                         end in
-          match req_opt with
-          | None => True
-          | Some req =>
-              let addr := mem_req_get_addr req in
-              (Bits.unsigned_le addr_min addr = true) /\ (Bits.unsigned_lt addr addr_max = true)
-          end.
-
-
-      Fixpoint prop_holds_for_sm_steps (steps: list step_params) (st: state)
-                                       (P: state -> Log R ContextEnv -> Log R ContextEnv -> Log R ContextEnv -> Prop) : Prop :=
-        match steps with
-        | [] => True
-        | step :: steps =>
-          let state' := do_step st step.(param_input) step.(param_feedback) in
-          prop_holds_about_sm_step st step P /\
-          prop_holds_for_sm_steps steps state' P
-        end.
-
-      Fixpoint valid_steps (st: state) (steps: list step_params) : Prop :=
-        match steps with
-        | [] => valid_input_state st
-        | step :: steps =>
-            let update := update_function st step.(param_input) in
-            let final := step.(param_feedback) update in
-            let state' := commit_update st final in
-            valid_input_log st step.(param_input) /\
-            valid_feedback_log st step.(param_input) final /\
-            valid_input_state state' /\
-            valid_steps state' steps
-        end.
-
-      (* If the core starts out in a limbo state, we say there are no valid writes to the outside world *)
-      Theorem limbo_implies_no_public_enqs:
-        forall (core_id: ind_core_id) (st: state) (log: Log R ContextEnv),
-        not (state_eq st core_id (value_of_bits Bits.zero)) ->
-        valid_input_state st ->
-        valid_input_log st log ->
-        no_public_enqs core_id st log.
-      Proof.
-      Admitted.
-
-      (* The proof itself is simpler, something like "output_is_a_function_of_partitioned_registers" *)
-      (* TODO: need to include mention of shared state *)
-      Theorem partitioned_when_in_reset_state:
-        forall (core_id: ind_core_id) (st: state) (eid: enclave_id),
-        valid_reset_state st core_id eid ->
-        forall (steps: list step_params),
-        valid_steps st steps ->
-        prop_holds_for_sm_steps steps st (P_no_enclave_req core_id) ->
-        prop_holds_for_sm_steps steps st (P_partition core_id).
-      Admitted.
-
-      Theorem reqs_to_enclave_memory_in_range:
-        forall (core_id: ind_core_id) (st: state) (eid: enclave_id),
-        valid_reset_state st core_id eid ->
-        forall (steps: list step_params),
-        valid_steps st steps ->
-        prop_holds_for_sm_steps steps st (P_no_enclave_req core_id) ->
-        prop_holds_for_sm_steps steps st (P_mem_reqs_in_range CacheType_Imem core_id eid) /\
-        prop_holds_for_sm_steps steps st (P_mem_reqs_in_range CacheType_Dmem core_id eid).
-      Admitted.
-
-      (* TODO: mention we are back in a reset state *)
-
-      (*
-      Variable input_fn : state -> Log R ContextEnv.
-      Variable pf_input_fn_generates_valid_log : forall (st: state), valid_input_log (input_fn st).
-      Variable feedback_fn : state -> Log R ContextEnv -> Log R ContextEnv.
-      Variable pf_feedback_fn_generates_valid_log
-        : forall (st: state) (log: Log R ContextEnv), valid_feedback_log st log (feedback_fn st log).
-
-      Definition do_step (st: state) : state :=
-        let input := input_fn st in
-        let update := update_function st input in
-        let final := feedback_fn st update in
-        commit_update st final.
-
-
-      Definition prop_holds_about_sm_step (st: state) (P: state -> Log R ContextEnv -> Log R ContextEnv -> Prop) : Prop :=
-        let input := input_fn st in
-        let update := update_function st input in
-        P st input update.
-
-      Fixpoint prop_holds_for_n_sm_steps (n: nat) (st: state) (P: state -> Log R ContextEnv -> Log R ContextEnv -> Prop) : Prop :=
-        match n with
-        | 0 => True
-        | S n' =>
-          let state' := do_step st in
-          prop_holds_about_sm_step st P /\
-          prop_holds_for_n_sm_steps n' state' P
-        end.
-
-      Definition P_partition (core_id: ind_core_id)
-                 (st: state) (input_log: Log R ContextEnv) (output_log: Log R ContextEnv) : Prop :=
-        forall st' log',
-        valid_input_state st' ->
-        valid_input_log log' ->
-        equiv_st_for_core core_id st st' ->
-        equiv_log_for_core core_id input_log log' ->
-        equiv_log_for_core core_id output_log (update_function st' log').
-
-      (* TODO: restructure *)
-      Definition observe_enclave_reqs (log: Log R ContextEnv) (core_id: ind_core_id) : option (struct_t enclave_req).
-      Admitted.
-
-      Definition valid_enclave_req (req: struct_t enclave_req) : Prop :=
-        let '(eid, _) := req in
-        Bits.to_nat eid < 4.
-
-      Definition P_no_enclave_req (core_id: ind_core_id): state -> Log R ContextEnv -> Log R ContextEnv -> Prop :=
-        fun st input_log output_log =>
-          match observe_enclave_reqs output_log core_id with
-          | None => True
-          | Some req => valid_enclave_req req
-          end.
-
-      (* TODO: stop duplicating code *)
-      Definition observe_imem_reqs_to_mem0 (log: Log R ContextEnv) : option (struct_t mem_req) :=
-        match latest_write0 log (toMem0_IMem MemReq.valid0) with
-        | Some b =>
-            if Bits.single b then (latest_write0 log (toMem0_IMem MemReq.data0)) else None
-        | None => None
-        end.
-
-      Definition observe_imem_reqs_to_mem1 (log: Log R ContextEnv) : option (struct_t mem_req) :=
-        match latest_write0 log (toMem1_IMem MemReq.valid0) with
-        | Some b =>
-            if Bits.single b then (latest_write0 log (toMem1_IMem MemReq.data0)) else None
-        | None => None
-        end.
-
-      Definition observe_imem_reqs_to_mem (log: Log R ContextEnv) (core_id: ind_core_id) : option (struct_t mem_req) :=
-        match core_id with
-        | CoreId0 => observe_imem_reqs_to_mem0 log
-        | CoreId1 => observe_imem_reqs_to_mem1 log
-        end.
-
-      Definition observe_dmem_reqs_to_mem0 (log: Log R ContextEnv) : option (struct_t mem_req) :=
-        match latest_write0 log (toMem0_DMem MemReq.valid0) with
-        | Some b =>
-            if Bits.single b then (latest_write0 log (toMem0_DMem MemReq.data0)) else None
-        | None => None
-        end.
-
-      Definition observe_dmem_reqs_to_mem1 (log: Log R ContextEnv) : option (struct_t mem_req) :=
-        match latest_write0 log (toMem1_DMem MemReq.valid0) with
-        | Some b =>
-            if Bits.single b then (latest_write0 log (toMem1_DMem MemReq.data0)) else None
-        | None => None
-        end.
-
-      Definition observe_dmem_reqs_to_mem (log: Log R ContextEnv) (core_id: ind_core_id) : option (struct_t mem_req) :=
-        match core_id with
-        | CoreId0 => observe_dmem_reqs_to_mem0 log
-        | CoreId1 => observe_dmem_reqs_to_mem1 log
-        end.
-
-      Definition P_mem_reqs_in_range (mem: ind_cache_type) (core_id: ind_core_id) (eid: enclave_id)
-                                     : state -> Log R ContextEnv -> Log R ContextEnv -> Prop :=
-        let addr_min := EnclaveParams.enclave_base eid in
-        let addr_max := Bits.plus (EnclaveParams.enclave_base eid) (EnclaveParams.enclave_size eid) in
-        fun st input_log output_log =>
-          let req_opt := match mem with
-                         | CacheType_Imem => observe_imem_reqs_to_mem output_log core_id
-                         | CacheType_Dmem => observe_dmem_reqs_to_mem output_log core_id
-                         end in
-          match req_opt with
-          | None => True
-          | Some req =>
-              let addr := mem_req_get_addr req in
-              (Bits.unsigned_le addr_min addr = true) /\ (Bits.unsigned_lt addr addr_max = true)
-          end.
-
-      (* The proof itself is simpler, something like "output_is_a_function_of_partitioned_registers" *)
-      (* TODO: need to include mention of shared state *)
-      Theorem partitioned_when_in_reset_state:
-        forall (core_id: ind_core_id) (st: state) (eid: enclave_id),
-        valid_reset_state st core_id eid ->
-        forall (n: nat),
-        prop_holds_for_n_sm_steps n st (P_no_enclave_req core_id) ->
-        prop_holds_for_n_sm_steps n st (P_partition core_id).
-      Admitted.
-
-      Theorem reqs_to_enclave_memory_in_range:
-        forall (core_id: ind_core_id) (st: state) (eid: enclave_id),
-        valid_reset_state st core_id eid ->
-        forall (n: nat),
-        prop_holds_for_n_sm_steps n st (P_no_enclave_req core_id) ->
-        prop_holds_for_n_sm_steps n st (P_mem_reqs_in_range CacheType_Imem core_id eid) /\
-        prop_holds_for_n_sm_steps n st (P_mem_reqs_in_range CacheType_Dmem core_id eid).
-      Admitted.
-
-      (* TODO: For context switching, state that core output is a function also of the other core's enclave *)
-      *)
-    End CycleModel.
-
-
-  End SMProperties.
-*)
-(*
-Module Pf (External: External_sig) (EnclaveParams: EnclaveParameters)
-          (Params0: CoreParameters) (Params1: CoreParameters)
-          (Core0: Core_sig External EnclaveParams Params0)
-          (Core1: Core_sig External EnclaveParams Params1)
-          (Memory: Memory_sig External).
-  Module Impl:= MachineSemantics External EnclaveParams Params0 Params1 Core0 Core1 Memory.
-  Import Common.
-  Import Interfaces.Common.
-
-  Record enclave_metadata :=
-    { meta_eid : enclave_id;
-      shared_page : bool
-    }.
-
-  Record enclave_params :=
-    { metadata : enclave_metadata;
-      param_dram: dram_t
-    }.
-
-  Record core_config : Type :=
-    { enclave_data : enclave_metadata;
-      in_limbo: bool;
-      requested_enclave: option enclave_metadata;
-      state_fn : nat -> observations_t
-    }.
-
-  Definition rf_t : Type := env_t ContextEnv Rf.R.
-
-  Definition isolated_function_t : Type := ind_core_id -> enclave_params -> rf_t -> nat -> observations_t.
-
-  Record partitioned_memory :=
-    { pm_enclave_mem : enclave_id -> option dram_t;
-      pm_shared_page : option dram_t;
-    }.
-
-  Record ghost_state :=
-    { core0_config : core_config;
-      core1_config : core_config;
-      mem_partitions : partitioned_memory;
-      num_cycles : nat
-    }.
-
-
-  (* TODO: This should be derived from Interfaces *)
-  Definition initial_rf : rf_t := ContextEnv.(create) Rf.r.
-
-  Definition mk_initial_config (fn: isolated_function_t) (core_id: ind_core_id)
-                               (params: enclave_params) (rf: rf_t) : core_config :=
-    {| enclave_data := params.(metadata);
-       in_limbo := false;
-       requested_enclave := None;
-       state_fn := fn core_id params rf
-    |}.
-
-  Definition enclave_base enc_id := Bits.to_nat (EnclaveParams.enclave_base enc_id).
-  Definition enclave_max enc_id := Bits.to_nat (Bits.plus (EnclaveParams.enclave_base enc_id)
-                                                          (EnclaveParams.enclave_size enc_id)).
-
-  Definition initial_enclave_dram initial_dram enc_id : dram_t :=
-    fun addr => if ((enclave_base enc_id) <=? addr) && (addr <? (enclave_max enc_id))
-             then initial_dram addr
-             else None.
-
-  Definition initial_shared_mem initial_dram : dram_t :=
-    fun addr => if ((Bits.to_nat (EnclaveParams.shared_mem_base) <=? addr) &&
-                 (addr <? Bits.to_nat (Bits.plus EnclaveParams.shared_mem_base EnclaveParams.shared_mem_size)))
-             then initial_dram addr
-             else None.
-
-  Definition mk_initial_pm (initial_dram: dram_t) : partitioned_memory :=
-    {| pm_enclave_mem := fun eid => Some (initial_enclave_dram initial_dram eid);
-       pm_shared_page := Some (initial_shared_mem initial_dram)
-    |}.
-
-  Definition initial_ghost_state (fn: isolated_function_t) (initial_dram: dram_t) : ghost_state :=
-    let enclave0_param :=
-        {| metadata := {| meta_eid := Enclave0;
-                          shared_page := false
-                       |};
-           param_dram := initial_enclave_dram initial_dram Enclave0
-        |} in
-    let enclave1_param :=
-        {| metadata := {| meta_eid := Enclave1;
-                          shared_page := false
-                       |};
-           param_dram := initial_enclave_dram initial_dram Enclave1
-        |} in
-    {| core0_config := mk_initial_config fn CoreId0 enclave0_param initial_rf;
-       core1_config := mk_initial_config fn CoreId1 enclave1_param initial_rf;
-       mem_partitions := {| pm_enclave_mem := fun eid => match eid with
-                                                      | (Enclave0 | Enclave1) => None
-                                                      | _ => Some (initial_enclave_dram initial_dram eid)
-                                                      end;
-                            pm_shared_page := Some (initial_shared_mem initial_dram)
-                         |};
-       num_cycles := 0
-    |}.
-
-  (* TODO: Do we care about cycle-accurate purge? *)
-  Inductive function_generates_trace_helper
-            (fn: isolated_function_t) (initial_dram: dram_t)
-            (ghost: ghost_state) (tr: trace) : Prop :=
-  | EmptyTrace :
-      forall (initial_ghost : ghost = initial_ghost_state fn initial_dram)
-        (empty_trace: tr = []),
-      function_generates_trace_helper fn initial_dram ghost tr
-  | IndTrace_BothRunning :
-      forall (prev_tr: trace) (obs: ind_core_id -> observations_t)
-        (prev_ghost: ghost_state) (ghost0 ghost1: ghost_state)
-
-        (* Induction hypothesis *)
-        (ind_hyp: function_generates_trace_helper fn initial_dram prev_ghost prev_tr)
-        (* If Core0 is running an enclave,
-         * fn must generate the relevant observation
-         *)
-        (pf_case_core0_running : prev_ghost.(core0_config).(in_limbo) = false ->
-                                 obs CoreId0 = prev_ghost.(core0_config).(state_fn) (S prev_ghost.(num_cycles))
-        )
-        (* If Core0 is not running an enclave *)
-        (pf_case_core0_limbo : prev_ghost.(core0_config).(in_limbo) = true ->
-                               obs CoreId0 = prev_ghost.(core0_config).(state_fn) (S prev_ghost.(num_cycles))
-        )
-
-
-        (* If Core1 is running an enclave *)
-        (* If Core1 is not running an enclave *)
-
-
-        (core0_running : prev_ghost.(core0_config).(in_limbo) = false)
-        (core1_running : prev_ghost.(core1_config).(in_limbo) = false)
-        (trace_eq: tr = prev_tr ++ [obs]),
-        (*
-        (ghost0_eq: ghost0 =
-        (ghost1_eq: ghost1 =
-
-        (cur_obs.obs_enclave_req
-        *)
-        (* TODO *)
-      function_generates_trace_helper fn initial_dram ghost tr.
-
-
-
-  Definition function_generates_trace (fn: isolated_function_t) (initial_dram: dram_t) (tr: trace) : Prop :=
-    exists ghost_state, function_generates_trace_helper fn initial_dram ghost_state tr.
-
-
-  Section Initialised.
-    Variable initial_dram: dram_t.
-
-    Theorem simulation: exists (iso_fn : isolated_function_t),
-      forall (n: nat) (impl_st: Impl.state) (impl_tr: trace),
-        Impl.step_n initial_dram n = (impl_st, impl_tr) ->
-        function_generates_trace iso_fn initial_dram impl_tr.
-    Admitted.
-
-  End Initialised.
-
-End Pf.
-*)
-
-(* TODO: move this *)
-
-*)
