examples/dynamic_isolation/RVCore.v
@@ -950,6 +950,10 @@ Module RV32I (EnclaveParams: EnclaveParameters) (CoreParams: CoreParameters)
   Parameter correctness : @P_correctness CoreParams.core_id CoreParams.initial_pc
                                          private_params External.ext
                                          rule_name_t rules schedule.
+  Parameter output_compliance : @P_output_compliance CoreParams.core_id CoreParams.initial_pc
+                                                     private_params External.ext
+                                                     rule_name_t rules schedule.
+
   Parameter compliance : @P_compliance CoreParams.core_id CoreParams.initial_pc
                                        private_params External.ext
                                        rule_name_t rules schedule.
