examples/dynamic_isolation/TrivialCore.v
@@ -63,6 +63,11 @@ Module EmptyCore (External: External_sig) (Params: EnclaveParameters) (CoreParam
   Parameter correctness : @Core_Common.P_correctness CoreParams.core_id CoreParams.initial_pc
                                                      private_params External.ext
                                                      rule_name_t rules schedule.
+  Parameter output_compliance :
+    @Core_Common.P_output_compliance CoreParams.core_id CoreParams.initial_pc
+                                     private_params External.ext
+                                     rule_name_t rules schedule.
+
   Parameter compliance : @Core_Common.P_compliance CoreParams.core_id CoreParams.initial_pc
                                                    private_params External.ext
                                                    rule_name_t rules schedule.
